@prefix : <http://purl.org/ontology/fo/> .
@prefix v: <http://rdf.data-vocabulary.org/#> .
@prefix dc: <http://purl.org/dc/elements/1.1/> .
@prefix fo: <http://purl.org/ontology/fo/> .
@prefix vs: <http://www.w3.org/2003/06/sw-vocab-status/ns#> .
@prefix owl: <http://www.w3.org/2002/07/owl#> .
@prefix rdf: <http://www.w3.org/1999/02/22-rdf-syntax-ns#> .
@prefix xml: <http://www.w3.org/XML/1998/namespace> .
@prefix xsd: <http://www.w3.org/2001/XMLSchema#> .
@prefix foaf: <http://xmlns.com/foaf/0.1/> .
@prefix rdfs: <http://www.w3.org/2000/01/rdf-schema#> .
@prefix skos: <http://www.w3.org/2004/02/skos/core#> .
@prefix dcmit: <http://purl.org/dc/dcmitype/> .
@prefix dcterms: <http://purl.org/dc/terms/> .
@prefix dctypes: <http://purl.org/dc/dcmitype/> .
@prefix provenance: <http://www.bbc.co.uk/ontologies/provenance/> .
@base <http://purl.org/ontology/fo/> .

<http://purl.org/ontology/fo/> rdf:type owl:Ontology ;
                                owl:versionIRI <http://purl.org/ontology/fo/1.1> ;
                                owl:imports provenance: ,
                                            vs: ,
                                            foaf: ;
                                dc:date "Date: 2014/03/18 16:30:00 " ;
                                provenance:canonicalLocation "https://repo.dev.bbc.co.uk/services/linked-data/ontologies/domain/kl/food/food-ontology-1-1.ttl"^^xsd:string ;
                                provenance:changeReason "Fix a typo of occassion"^^xsd:string ;
                                provenance:public "true"^^xsd:boolean ;
                                provenance:slug "fo"^^xsd:string ;
                                provenance:version "1.1"^^xsd:double ;
                                rdfs:comment "A simple vocabulary for describing recipes, ingredients, menus and diets."@en-gb ;
                                rdfs:label "Food Ontology"^^xsd:string ;
                                owl:priorVersion <http://purl.org/ontology/fo/1.0> .

#################################################################
#    Annotation properties
#################################################################

###  http://purl.org/dc/elements/1.1/contributor
dc:contributor dcterms:description "Examples of a Contributor include a person, an organization, or a service. Typically, the name of a Contributor should be used to indicate the entity."@en ;
               dcterms:hasVersion <http://dublincore.org/usage/terms/history/#contributor-006> ;
               dcterms:issued "1999-07-02"^^xsd:date ;
               dcterms:modified "2008-01-14"^^xsd:date ;
               rdfs:comment "An entity responsible for making contributions to the resource."@en ;
               rdfs:isDefinedBy dc: ;
               rdfs:label "Contributor"@en ;
               skos:note "A second property with the same name as this property has been declared in the dcterms: namespace (http://purl.org/dc/terms/).  See the Introduction to the document \"DCMI Metadata Terms\" (http://dublincore.org/documents/dcmi-terms/) for an explanation."@en .


###  http://purl.org/dc/elements/1.1/coverage
dc:coverage rdf:type owl:AnnotationProperty ;
            dcterms:description "Spatial topic and spatial applicability may be a named place or a location specified by its geographic coordinates. Temporal topic may be a named period, date, or date range. A jurisdiction may be a named administrative entity or a geographic place to which the resource applies. Recommended best practice is to use a controlled vocabulary such as the Thesaurus of Geographic Names [TGN]. Where appropriate, named places or time periods can be used in preference to numeric identifiers such as sets of coordinates or date ranges."@en ;
            dcterms:hasVersion <http://dublincore.org/usage/terms/history/#coverage-006> ;
            dcterms:issued "1999-07-02"^^xsd:date ;
            dcterms:modified "2008-01-14"^^xsd:date ;
            rdfs:comment "The spatial or temporal topic of the resource, the spatial applicability of the resource, or the jurisdiction under which the resource is relevant."@en ;
            rdfs:isDefinedBy dc: ;
            rdfs:label "Coverage"@en ;
            skos:note "A second property with the same name as this property has been declared in the dcterms: namespace (http://purl.org/dc/terms/).  See the Introduction to the document \"DCMI Metadata Terms\" (http://dublincore.org/documents/dcmi-terms/) for an explanation."@en .


###  http://purl.org/dc/elements/1.1/creator
dc:creator dcterms:description "Examples of a Creator include a person, an organization, or a service. Typically, the name of a Creator should be used to indicate the entity."@en ;
           dcterms:hasVersion <http://dublincore.org/usage/terms/history/#creator-006> ;
           dcterms:issued "1999-07-02"^^xsd:date ;
           dcterms:modified "2008-01-14"^^xsd:date ;
           rdfs:comment "An entity primarily responsible for making the resource."@en ;
           rdfs:isDefinedBy dc: ;
           rdfs:label "Creator"@en ;
           skos:note "A second property with the same name as this property has been declared in the dcterms: namespace (http://purl.org/dc/terms/).  See the Introduction to the document \"DCMI Metadata Terms\" (http://dublincore.org/documents/dcmi-terms/) for an explanation."@en .


###  http://purl.org/dc/elements/1.1/date
dc:date dcterms:description "Date may be used to express temporal information at any level of granularity.  Recommended best practice is to use an encoding scheme, such as the W3CDTF profile of ISO 8601 [W3CDTF]."@en ;
        dcterms:hasVersion <http://dublincore.org/usage/terms/history/#date-006> ;
        dcterms:issued "1999-07-02"^^xsd:date ;
        dcterms:modified "2008-01-14"^^xsd:date ;
        rdfs:comment "A point or period of time associated with an event in the lifecycle of the resource."@en ;
        rdfs:isDefinedBy dc: ;
        rdfs:label "Date"@en ;
        skos:note "A second property with the same name as this property has been declared in the dcterms: namespace (http://purl.org/dc/terms/).  See the Introduction to the document \"DCMI Metadata Terms\" (http://dublincore.org/documents/dcmi-terms/) for an explanation."@en .


###  http://purl.org/dc/elements/1.1/description
dc:description dcterms:description "Description may include but is not limited to: an abstract, a table of contents, a graphical representation, or a free-text account of the resource."@en ;
               dcterms:hasVersion <http://dublincore.org/usage/terms/history/#description-006> ;
               dcterms:issued "1999-07-02"^^xsd:date ;
               dcterms:modified "2008-01-14"^^xsd:date ;
               rdfs:comment "An account of the resource."@en ;
               rdfs:isDefinedBy dc: ;
               rdfs:label "Description"@en ;
               skos:note "A second property with the same name as this property has been declared in the dcterms: namespace (http://purl.org/dc/terms/).  See the Introduction to the document \"DCMI Metadata Terms\" (http://dublincore.org/documents/dcmi-terms/) for an explanation."@en .


###  http://purl.org/dc/elements/1.1/format
dc:format rdf:type owl:AnnotationProperty ;
          dcterms:description "Examples of dimensions include size and duration. Recommended best practice is to use a controlled vocabulary such as the list of Internet Media Types [MIME]."@en ;
          dcterms:hasVersion <http://dublincore.org/usage/terms/history/#format-007> ;
          dcterms:issued "1999-07-02"^^xsd:date ;
          dcterms:modified "2008-01-14"^^xsd:date ;
          rdfs:comment "The file format, physical medium, or dimensions of the resource."@en ;
          rdfs:isDefinedBy dc: ;
          rdfs:label "Format"@en ;
          skos:note "A second property with the same name as this property has been declared in the dcterms: namespace (http://purl.org/dc/terms/).  See the Introduction to the document \"DCMI Metadata Terms\" (http://dublincore.org/documents/dcmi-terms/) for an explanation."@en .


###  http://purl.org/dc/elements/1.1/identifier
dc:identifier rdf:type owl:AnnotationProperty ;
              dcterms:description "Recommended best practice is to identify the resource by means of a string conforming to a formal identification system. "@en ;
              dcterms:hasVersion <http://dublincore.org/usage/terms/history/#identifier-006> ;
              dcterms:issued "1999-07-02"^^xsd:date ;
              dcterms:modified "2008-01-14"^^xsd:date ;
              rdfs:comment "An unambiguous reference to the resource within a given context."@en ;
              rdfs:isDefinedBy dc: ;
              rdfs:label "Identifier"@en ;
              skos:note "A second property with the same name as this property has been declared in the dcterms: namespace (http://purl.org/dc/terms/).  See the Introduction to the document \"DCMI Metadata Terms\" (http://dublincore.org/documents/dcmi-terms/) for an explanation."@en .


###  http://purl.org/dc/elements/1.1/language
dc:language rdf:type owl:AnnotationProperty ;
            dcterms:description "Recommended best practice is to use a controlled vocabulary such as RFC 4646 [RFC4646]."@en ;
            dcterms:hasVersion <http://dublincore.org/usage/terms/history/#language-007> ;
            dcterms:issued "1999-07-02"^^xsd:date ;
            dcterms:modified "2008-01-14"^^xsd:date ;
            rdfs:comment "A language of the resource."@en ;
            rdfs:isDefinedBy dc: ;
            rdfs:label "Language"@en ;
            rdfs:seeAlso <http://www.ietf.org/rfc/rfc4646.txt> ;
            skos:note "A second property with the same name as this property has been declared in the dcterms: namespace (http://purl.org/dc/terms/).  See the Introduction to the document \"DCMI Metadata Terms\" (http://dublincore.org/documents/dcmi-terms/) for an explanation."@en .


###  http://purl.org/dc/elements/1.1/publisher
dc:publisher rdf:type owl:AnnotationProperty ;
             dcterms:description "Examples of a Publisher include a person, an organization, or a service. Typically, the name of a Publisher should be used to indicate the entity."@en ;
             dcterms:hasVersion <http://dublincore.org/usage/terms/history/#publisher-006> ;
             dcterms:issued "1999-07-02"^^xsd:date ;
             dcterms:modified "2008-01-14"^^xsd:date ;
             rdfs:comment "An entity responsible for making the resource available."@en ;
             rdfs:isDefinedBy dc: ;
             rdfs:label "Publisher"@en ;
             skos:note "A second property with the same name as this property has been declared in the dcterms: namespace (http://purl.org/dc/terms/).  See the Introduction to the document \"DCMI Metadata Terms\" (http://dublincore.org/documents/dcmi-terms/) for an explanation."@en .


###  http://purl.org/dc/elements/1.1/relation
dc:relation rdf:type owl:AnnotationProperty ;
            dcterms:description "Recommended best practice is to identify the related resource by means of a string conforming to a formal identification system. "@en ;
            dcterms:hasVersion <http://dublincore.org/usage/terms/history/#relation-006> ;
            dcterms:issued "1999-07-02"^^xsd:date ;
            dcterms:modified "2008-01-14"^^xsd:date ;
            rdfs:comment "A related resource."@en ;
            rdfs:isDefinedBy dc: ;
            rdfs:label "Relation"@en ;
            skos:note "A second property with the same name as this property has been declared in the dcterms: namespace (http://purl.org/dc/terms/).  See the Introduction to the document \"DCMI Metadata Terms\" (http://dublincore.org/documents/dcmi-terms/) for an explanation."@en .


###  http://purl.org/dc/elements/1.1/rights
dc:rights rdf:type owl:AnnotationProperty ;
          dcterms:description "Typically, rights information includes a statement about various property rights associated with the resource, including intellectual property rights."@en ;
          dcterms:hasVersion <http://dublincore.org/usage/terms/history/#rights-006> ;
          dcterms:issued "1999-07-02"^^xsd:date ;
          dcterms:modified "2008-01-14"^^xsd:date ;
          rdfs:comment "Information about rights held in and over the resource."@en ;
          rdfs:isDefinedBy dc: ;
          rdfs:label "Rights"@en ;
          skos:note "A second property with the same name as this property has been declared in the dcterms: namespace (http://purl.org/dc/terms/).  See the Introduction to the document \"DCMI Metadata Terms\" (http://dublincore.org/documents/dcmi-terms/) for an explanation."@en .


###  http://purl.org/dc/elements/1.1/source
dc:source rdf:type owl:AnnotationProperty ;
          dcterms:description "The described resource may be derived from the related resource in whole or in part. Recommended best practice is to identify the related resource by means of a string conforming to a formal identification system."@en ;
          dcterms:hasVersion <http://dublincore.org/usage/terms/history/#source-006> ;
          dcterms:issued "1999-07-02"^^xsd:date ;
          dcterms:modified "2008-01-14"^^xsd:date ;
          rdfs:comment "A related resource from which the described resource is derived."@en ;
          rdfs:isDefinedBy dc: ;
          rdfs:label "Source"@en ;
          skos:note "A second property with the same name as this property has been declared in the dcterms: namespace (http://purl.org/dc/terms/).  See the Introduction to the document \"DCMI Metadata Terms\" (http://dublincore.org/documents/dcmi-terms/) for an explanation."@en .


###  http://purl.org/dc/elements/1.1/subject
dc:subject rdf:type owl:AnnotationProperty ;
           dcterms:description "Typically, the subject will be represented using keywords, key phrases, or classification codes. Recommended best practice is to use a controlled vocabulary."@en ;
           dcterms:hasVersion <http://dublincore.org/usage/terms/history/#subject-007> ;
           dcterms:issued "1999-07-02"^^xsd:date ;
           dcterms:modified "2012-06-14"^^xsd:date ;
           rdfs:comment "The topic of the resource."@en ;
           rdfs:isDefinedBy dc: ;
           rdfs:label "Subject"@en ;
           skos:note "A second property with the same name as this property has been declared in the dcterms: namespace (http://purl.org/dc/terms/).  See the Introduction to the document \"DCMI Metadata Terms\" (http://dublincore.org/documents/dcmi-terms/) for an explanation."@en .


###  http://purl.org/dc/elements/1.1/title
dc:title dcterms:hasVersion <http://dublincore.org/usage/terms/history/#title-006> ;
         dcterms:issued "1999-07-02"^^xsd:date ;
         dcterms:modified "2008-01-14"^^xsd:date ;
         rdfs:comment "A name given to the resource."@en ;
         rdfs:isDefinedBy dc: ;
         rdfs:label "Title"@en ;
         skos:note "A second property with the same name as this property has been declared in the dcterms: namespace (http://purl.org/dc/terms/).  See the Introduction to the document \"DCMI Metadata Terms\" (http://dublincore.org/documents/dcmi-terms/) for an explanation."@en .


###  http://purl.org/dc/elements/1.1/type
dc:type rdf:type owl:AnnotationProperty ;
        dcterms:description "Recommended best practice is to use a controlled vocabulary such as the DCMI Type Vocabulary [DCMITYPE]. To describe the file format, physical medium, or dimensions of the resource, use the Format element."@en ;
        dcterms:hasVersion <http://dublincore.org/usage/terms/history/#type-006> ;
        dcterms:issued "1999-07-02"^^xsd:date ;
        dcterms:modified "2008-01-14"^^xsd:date ;
        rdfs:comment "The nature or genre of the resource."@en ;
        rdfs:isDefinedBy dc: ;
        rdfs:label "Type"@en ;
        skos:note "A second property with the same name as this property has been declared in the dcterms: namespace (http://purl.org/dc/terms/).  See the Introduction to the document \"DCMI Metadata Terms\" (http://dublincore.org/documents/dcmi-terms/) for an explanation."@en .


###  http://purl.org/dc/terms/abstract
dcterms:abstract rdf:type owl:AnnotationProperty ;
                 rdfs:subPropertyOf dc:description ,
                                    dcterms:description .


###  http://purl.org/dc/terms/accessRights
dcterms:accessRights rdf:type owl:AnnotationProperty ;
                     rdfs:subPropertyOf dc:rights .


###  http://purl.org/dc/terms/alternative
dcterms:alternative rdf:type owl:AnnotationProperty ;
                    rdfs:subPropertyOf dc:title .


###  http://purl.org/dc/terms/available
dcterms:available rdf:type owl:AnnotationProperty ;
                  rdfs:subPropertyOf dc:date .


###  http://purl.org/dc/terms/bibliographicCitation
dcterms:bibliographicCitation rdf:type owl:AnnotationProperty ;
                              rdfs:subPropertyOf dc:identifier .


###  http://purl.org/dc/terms/conformsTo
dcterms:conformsTo rdf:type owl:AnnotationProperty ;
                   rdfs:subPropertyOf dc:relation ,
                                      dcterms:relation .


###  http://purl.org/dc/terms/contributor
dcterms:contributor rdf:type owl:AnnotationProperty ;
                    rdfs:subPropertyOf dc:contributor .


###  http://purl.org/dc/terms/coverage
dcterms:coverage rdf:type owl:AnnotationProperty ;
                 rdfs:subPropertyOf dc:coverage .


###  http://purl.org/dc/terms/created
dcterms:created rdf:type owl:AnnotationProperty ;
                rdfs:subPropertyOf dc:date .


###  http://purl.org/dc/terms/creator
dcterms:creator rdf:type owl:AnnotationProperty ;
                rdfs:subPropertyOf dc:creator .


###  http://purl.org/dc/terms/date
dcterms:date rdf:type owl:AnnotationProperty ;
             rdfs:subPropertyOf dc:date .


###  http://purl.org/dc/terms/dateAccepted
dcterms:dateAccepted rdf:type owl:AnnotationProperty ;
                     rdfs:subPropertyOf dc:date .


###  http://purl.org/dc/terms/dateCopyrighted
dcterms:dateCopyrighted rdf:type owl:AnnotationProperty ;
                        rdfs:subPropertyOf dc:date .


###  http://purl.org/dc/terms/dateSubmitted
dcterms:dateSubmitted rdf:type owl:AnnotationProperty ;
                      rdfs:subPropertyOf dc:date .


###  http://purl.org/dc/terms/description
dcterms:description rdf:type owl:AnnotationProperty ;
                    rdfs:subPropertyOf dc:description .


###  http://purl.org/dc/terms/extent
dcterms:extent rdf:type owl:AnnotationProperty ;
               rdfs:subPropertyOf dc:format .


###  http://purl.org/dc/terms/format
dcterms:format rdf:type owl:AnnotationProperty ;
               rdfs:subPropertyOf dc:format .


###  http://purl.org/dc/terms/hasFormat
dcterms:hasFormat rdf:type owl:AnnotationProperty ;
                  rdfs:subPropertyOf dc:relation ,
                                     dcterms:relation .


###  http://purl.org/dc/terms/hasPart
dcterms:hasPart rdf:type owl:AnnotationProperty ;
                rdfs:subPropertyOf dc:relation ,
                                   dcterms:relation .


###  http://purl.org/dc/terms/hasVersion
dcterms:hasVersion rdf:type owl:AnnotationProperty ;
                   rdfs:subPropertyOf dc:relation ,
                                      dcterms:relation .


###  http://purl.org/dc/terms/identifier
dcterms:identifier rdf:type owl:AnnotationProperty ;
                   rdfs:subPropertyOf dc:identifier .


###  http://purl.org/dc/terms/isFormatOf
dcterms:isFormatOf rdf:type owl:AnnotationProperty ;
                   rdfs:subPropertyOf dc:relation ,
                                      dcterms:relation .


###  http://purl.org/dc/terms/isPartOf
dcterms:isPartOf rdf:type owl:AnnotationProperty ;
                 rdfs:subPropertyOf dc:relation ,
                                    dcterms:relation .


###  http://purl.org/dc/terms/isReferencedBy
dcterms:isReferencedBy rdf:type owl:AnnotationProperty ;
                       rdfs:subPropertyOf dc:relation ,
                                          dcterms:relation .


###  http://purl.org/dc/terms/isReplacedBy
dcterms:isReplacedBy rdf:type owl:AnnotationProperty ;
                     rdfs:subPropertyOf dc:relation ,
                                        dcterms:relation .


###  http://purl.org/dc/terms/isRequiredBy
dcterms:isRequiredBy rdf:type owl:AnnotationProperty ;
                     rdfs:subPropertyOf dc:relation ,
                                        dcterms:relation .


###  http://purl.org/dc/terms/isVersionOf
dcterms:isVersionOf rdf:type owl:AnnotationProperty ;
                    rdfs:subPropertyOf dc:relation ,
                                       dcterms:relation .


###  http://purl.org/dc/terms/issued
dcterms:issued rdf:type owl:AnnotationProperty ;
               rdfs:subPropertyOf dc:date .


###  http://purl.org/dc/terms/language
dcterms:language rdf:type owl:AnnotationProperty ;
                 rdfs:subPropertyOf dc:language .


###  http://purl.org/dc/terms/license
dcterms:license rdf:type owl:AnnotationProperty ;
                rdfs:subPropertyOf dc:rights .


###  http://purl.org/dc/terms/medium
dcterms:medium rdf:type owl:AnnotationProperty ;
               rdfs:subPropertyOf dc:format .


###  http://purl.org/dc/terms/modified
dcterms:modified rdf:type owl:AnnotationProperty ;
                 rdfs:subPropertyOf dc:date .


###  http://purl.org/dc/terms/publisher
dcterms:publisher rdf:type owl:AnnotationProperty ;
                  rdfs:subPropertyOf dc:publisher .


###  http://purl.org/dc/terms/references
dcterms:references rdf:type owl:AnnotationProperty ;
                   rdfs:subPropertyOf dc:relation ,
                                      dcterms:relation .


###  http://purl.org/dc/terms/relation
dcterms:relation rdf:type owl:AnnotationProperty ;
                 rdfs:subPropertyOf dc:relation .


###  http://purl.org/dc/terms/replaces
dcterms:replaces rdf:type owl:AnnotationProperty ;
                 rdfs:subPropertyOf dc:relation ,
                                    dcterms:relation .


###  http://purl.org/dc/terms/requires
dcterms:requires rdf:type owl:AnnotationProperty ;
                 rdfs:subPropertyOf dc:relation ,
                                    dcterms:relation .


###  http://purl.org/dc/terms/rights
dcterms:rights rdf:type owl:AnnotationProperty ;
               rdfs:subPropertyOf dc:rights .


###  http://purl.org/dc/terms/source
dcterms:source rdf:type owl:AnnotationProperty ;
               rdfs:subPropertyOf dc:source ,
                                  dcterms:relation .


###  http://purl.org/dc/terms/spatial
dcterms:spatial rdf:type owl:AnnotationProperty ;
                rdfs:subPropertyOf dc:coverage .


###  http://purl.org/dc/terms/subject
dcterms:subject rdf:type owl:AnnotationProperty ;
                rdfs:subPropertyOf dc:subject .


###  http://purl.org/dc/terms/tableOfContents
dcterms:tableOfContents rdf:type owl:AnnotationProperty ;
                        rdfs:subPropertyOf dc:description ,
                                           dcterms:description .


###  http://purl.org/dc/terms/temporal
dcterms:temporal rdf:type owl:AnnotationProperty ;
                 rdfs:subPropertyOf dc:coverage .


###  http://purl.org/dc/terms/title
dcterms:title rdf:type owl:AnnotationProperty ;
              rdfs:subPropertyOf dc:title .


###  http://purl.org/dc/terms/type
dcterms:type rdf:type owl:AnnotationProperty ;
             rdfs:subPropertyOf dc:type .


###  http://purl.org/dc/terms/valid
dcterms:valid rdf:type owl:AnnotationProperty ;
              rdfs:subPropertyOf dc:date .


###  http://www.bbc.co.uk/ontologies/provenance/canonicalLocation
provenance:canonicalLocation rdf:type owl:AnnotationProperty .


###  http://www.bbc.co.uk/ontologies/provenance/changeReason
provenance:changeReason rdf:type owl:AnnotationProperty .


###  http://www.bbc.co.uk/ontologies/provenance/public
provenance:public rdf:type owl:AnnotationProperty .


###  http://www.bbc.co.uk/ontologies/provenance/slug
provenance:slug rdf:type owl:AnnotationProperty .


###  http://www.bbc.co.uk/ontologies/provenance/version
provenance:version rdf:type owl:AnnotationProperty .


###  http://www.w3.org/2004/02/skos/core#note
skos:note rdf:type owl:AnnotationProperty .


#################################################################
#    Datatypes
#################################################################

###  http://purl.org/dc/terms/Box
dcterms:Box rdf:type rdfs:Datatype .


###  http://purl.org/dc/terms/ISO3166
dcterms:ISO3166 rdf:type rdfs:Datatype .


###  http://purl.org/dc/terms/ISO639-2
dcterms:ISO639-2 rdf:type rdfs:Datatype .


###  http://purl.org/dc/terms/ISO639-3
dcterms:ISO639-3 rdf:type rdfs:Datatype .


###  http://purl.org/dc/terms/Period
dcterms:Period rdf:type rdfs:Datatype .


###  http://purl.org/dc/terms/Point
dcterms:Point rdf:type rdfs:Datatype .


###  http://purl.org/dc/terms/RFC1766
dcterms:RFC1766 rdf:type rdfs:Datatype .


###  http://purl.org/dc/terms/RFC3066
dcterms:RFC3066 rdf:type rdfs:Datatype .


###  http://purl.org/dc/terms/RFC4646
dcterms:RFC4646 rdf:type rdfs:Datatype .


###  http://purl.org/dc/terms/RFC5646
dcterms:RFC5646 rdf:type rdfs:Datatype .


###  http://purl.org/dc/terms/URI
dcterms:URI rdf:type rdfs:Datatype .


###  http://purl.org/dc/terms/W3CDTF
dcterms:W3CDTF rdf:type rdfs:Datatype .


###  http://www.w3.org/2001/XMLSchema#date
xsd:date rdf:type rdfs:Datatype .


#################################################################
#    Object Properties
#################################################################

###  http://purl.org/dc/terms/accessRights
dcterms:accessRights rdf:type owl:ObjectProperty ;
                     rdfs:subPropertyOf dcterms:rights ;
                     rdfs:range dcterms:RightsStatement .


###  http://purl.org/dc/terms/accrualMethod
dcterms:accrualMethod rdf:type owl:ObjectProperty ;
                      rdfs:domain dctypes:Collection ;
                      rdfs:range dcterms:MethodOfAccrual .


###  http://purl.org/dc/terms/accrualPeriodicity
dcterms:accrualPeriodicity rdf:type owl:ObjectProperty ;
                           rdfs:domain dctypes:Collection ;
                           rdfs:range dcterms:Frequency .


###  http://purl.org/dc/terms/accrualPolicy
dcterms:accrualPolicy rdf:type owl:ObjectProperty ;
                      rdfs:domain dctypes:Collection ;
                      rdfs:range dcterms:Policy .


###  http://purl.org/dc/terms/audience
dcterms:audience rdf:type owl:ObjectProperty ;
                 rdfs:range dcterms:AgentClass .


###  http://purl.org/dc/terms/conformsTo
dcterms:conformsTo rdf:type owl:ObjectProperty ;
                   rdfs:range dcterms:Standard .


###  http://purl.org/dc/terms/contributor
dcterms:contributor rdf:type owl:ObjectProperty ;
                    rdfs:range dcterms:Agent .


###  http://purl.org/dc/terms/coverage
dcterms:coverage rdf:type owl:ObjectProperty ;
                 rdfs:range dcterms:LocationPeriodOrJurisdiction .


###  http://purl.org/dc/terms/creator
dcterms:creator rdf:type owl:ObjectProperty ;
                rdfs:subPropertyOf dcterms:contributor ;
                rdfs:range dcterms:Agent .


###  http://purl.org/dc/terms/educationLevel
dcterms:educationLevel rdf:type owl:ObjectProperty ;
                       rdfs:subPropertyOf dcterms:audience ;
                       rdfs:range dcterms:AgentClass .


###  http://purl.org/dc/terms/extent
dcterms:extent rdf:type owl:ObjectProperty ;
               rdfs:subPropertyOf dcterms:format ;
               rdfs:range dcterms:SizeOrDuration .


###  http://purl.org/dc/terms/format
dcterms:format rdf:type owl:ObjectProperty ;
               rdfs:range dcterms:MediaTypeOrExtent .


###  http://purl.org/dc/terms/instructionalMethod
dcterms:instructionalMethod rdf:type owl:ObjectProperty ;
                            rdfs:range dcterms:MethodOfInstruction .


###  http://purl.org/dc/terms/language
dcterms:language rdf:type owl:ObjectProperty ;
                 rdfs:range dcterms:LinguisticSystem .


###  http://purl.org/dc/terms/license
dcterms:license rdf:type owl:ObjectProperty ;
                rdfs:subPropertyOf dcterms:rights ;
                rdfs:range dcterms:LicenseDocument .


###  http://purl.org/dc/terms/mediator
dcterms:mediator rdf:type owl:ObjectProperty ;
                 rdfs:subPropertyOf dcterms:audience ;
                 rdfs:range dcterms:AgentClass .


###  http://purl.org/dc/terms/medium
dcterms:medium rdf:type owl:ObjectProperty ;
               rdfs:subPropertyOf dcterms:format ;
               rdfs:domain dcterms:PhysicalResource ;
               rdfs:range dcterms:PhysicalMedium .


###  http://purl.org/dc/terms/provenance
dcterms:provenance rdf:type owl:ObjectProperty ;
                   rdfs:range dcterms:ProvenanceStatement .


###  http://purl.org/dc/terms/publisher
dcterms:publisher rdf:type owl:ObjectProperty ;
                  rdfs:range dcterms:Agent .


###  http://purl.org/dc/terms/rights
dcterms:rights rdf:type owl:ObjectProperty ;
               rdfs:range dcterms:RightsStatement .


###  http://purl.org/dc/terms/rightsHolder
dcterms:rightsHolder rdf:type owl:ObjectProperty ;
                     rdfs:range dcterms:Agent .


###  http://purl.org/dc/terms/spatial
dcterms:spatial rdf:type owl:ObjectProperty ;
                rdfs:subPropertyOf dcterms:coverage ;
                rdfs:range dcterms:Location .


###  http://purl.org/dc/terms/temporal
dcterms:temporal rdf:type owl:ObjectProperty ;
                 rdfs:subPropertyOf dcterms:coverage ;
                 rdfs:range dcterms:PeriodOfTime .


###  http://purl.org/dc/terms/type
dcterms:type rdf:type owl:ObjectProperty ;
             rdfs:range rdfs:Class .


###  http://purl.org/ontology/fo/at_its_best
fo:at_its_best rdf:type owl:ObjectProperty ;
               rdfs:domain fo:Food ;
               rdfs:range fo:Season ;
               rdfs:comment "The at its best property tells us in what season a particular food is at its best."@en-gb ;
               rdfs:isDefinedBy <http://purl.org/ontology/fo/> ;
               rdfs:label "at its best"@en-gb ;
               vs:term_status "testing" .


###  http://purl.org/ontology/fo/canape
fo:canape rdf:type owl:ObjectProperty ;
          rdfs:domain fo:Menu ;
          rdfs:range fo:Recipe ;
          rdfs:comment "The canape property relates a menu to a recipe that may be served as a canape."@en-gb ;
          rdfs:isDefinedBy <http://purl.org/ontology/fo/> ;
          rdfs:label "canape"@en-gb ;
          vs:term_status "testing" .


###  http://purl.org/ontology/fo/cuisine
fo:cuisine rdf:type owl:ObjectProperty ;
           rdfs:domain fo:Recipe ;
           rdfs:range fo:Cuisine ;
           rdfs:comment "The cuisine property classifies a recipe as being an example of that cuisine."@en-gb ;
           rdfs:isDefinedBy <http://purl.org/ontology/fo/> ;
           rdfs:label "cuisine"@en-gb ;
           vs:term_status "testing" .


###  http://purl.org/ontology/fo/dessert
fo:dessert rdf:type owl:ObjectProperty ;
           rdfs:domain fo:Menu ;
           rdfs:range fo:Recipe ;
           rdfs:comment "The dessert property relates a menu to a recipe that may be served as a dessert."@en-gb ;
           rdfs:isDefinedBy <http://purl.org/ontology/fo/> ;
           rdfs:label "dessert"@en-gb ;
           vs:term_status "testing" .


###  http://purl.org/ontology/fo/diet
fo:diet rdf:type owl:ObjectProperty ;
        rdfs:domain fo:Recipe ;
        rdfs:range fo:Diet ;
        rdfs:comment "The diet property relates a recipe to a diet it may be suitable for."@en-gb ;
        rdfs:isDefinedBy <http://purl.org/ontology/fo/> ;
        rdfs:label "diet"@en-gb ;
        vs:term_status "testing" .


###  http://purl.org/ontology/fo/food
fo:food rdf:type owl:ObjectProperty ;
        rdfs:domain fo:Ingredient ;
        rdfs:range fo:Food ;
        rdfs:comment "The food property relates an ingredient to the food that is required."@en-gb ;
        rdfs:isDefinedBy <http://purl.org/ontology/fo/> ;
        rdfs:label "food"@en-gb ;
        vs:term_status "testing" .


###  http://purl.org/ontology/fo/ingredients
fo:ingredients rdf:type owl:ObjectProperty ;
               rdfs:range fo:IngredientList ;
               rdfs:comment "The ingredients property relates a recipe or recipe stage to an ingredient list."@en-gb ;
               rdfs:isDefinedBy <http://purl.org/ontology/fo/> ;
               rdfs:label "ingredients"@en-gb ;
               vs:term_status "testing" .


###  http://purl.org/ontology/fo/main_course
fo:main_course rdf:type owl:ObjectProperty ;
               rdfs:domain fo:Menu ;
               rdfs:range fo:Recipe ;
               rdfs:comment "The main course property relates a menu to a recipe that may be served as a main course."@en-gb ;
               rdfs:isDefinedBy <http://purl.org/ontology/fo/> ;
               rdfs:label "main course"@en-gb ;
               vs:term_status "testing" .


###  http://purl.org/ontology/fo/method
fo:method rdf:type owl:ObjectProperty ;
          rdfs:range fo:Method ;
          rdfs:comment "The method property relates a recipe or stage to the method used to make it."@en-gb ;
          rdfs:isDefinedBy <http://purl.org/ontology/fo/> ;
          rdfs:label "method"@en-gb ;
          vs:term_status "testing" .


###  http://purl.org/ontology/fo/occasion
fo:occasion rdf:type owl:ObjectProperty ;
            rdfs:domain fo:Recipe ;
            rdfs:range fo:Occasion ;
            rdfs:comment "The occassion property relates a recipe to an occasion it may be appropriate for."@en-gb ;
            rdfs:isDefinedBy <http://purl.org/ontology/fo/> ;
            rdfs:label "occassion"@en-gb ;
            vs:term_status "testing" .


###  http://purl.org/ontology/fo/produces
fo:produces rdf:type owl:ObjectProperty ;
            rdfs:domain fo:Recipe ;
            rdfs:range fo:Food ;
            rdfs:comment "The produces property relates a recipe to the food it produces."@en-gb ;
            rdfs:isDefinedBy <http://purl.org/ontology/fo/> ;
            rdfs:label "produces"@en-gb ;
            vs:term_status "testing" .


###  http://purl.org/ontology/fo/required_technique
fo:required_technique rdf:type owl:ObjectProperty ;
                      rdfs:range fo:Technique ;
                      rdfs:comment "The required technique property indicates that a particular technique is required in order to complete a recipe, method or step."@en-gb ;
                      rdfs:isDefinedBy <http://purl.org/ontology/fo/> ;
                      rdfs:label "required technique"@en-gb ;
                      vs:term_status "testing" .


###  http://purl.org/ontology/fo/serve_as
fo:serve_as rdf:type owl:ObjectProperty ;
            rdfs:domain fo:Recipe ;
            rdfs:range fo:Course ;
            rdfs:comment "The serve as property relates a recipe to the course in a meal that it may be served as."@en-gb ;
            rdfs:isDefinedBy <http://purl.org/ontology/fo/> ;
            rdfs:label "serve as"@en-gb ;
            vs:term_status "testing" .


###  http://purl.org/ontology/fo/shopping_category
fo:shopping_category rdf:type owl:ObjectProperty ;
                     rdfs:domain fo:Food ;
                     rdfs:range fo:ShoppingCategory ;
                     rdfs:comment "The shopping category property relates a food to the shopping category where that food is likely to be found when shopping for it."@en-gb ;
                     rdfs:isDefinedBy <http://purl.org/ontology/fo/> ;
                     rdfs:label "shopping category"@en-gb ;
                     vs:term_status "testing" .


###  http://purl.org/ontology/fo/side_dish
fo:side_dish rdf:type owl:ObjectProperty ;
             rdfs:domain fo:Menu ;
             rdfs:range fo:Recipe ;
             rdfs:comment "The side dish property relates a menu to a recipe that may be served as a side dish."@en-gb ;
             rdfs:isDefinedBy <http://purl.org/ontology/fo/> ;
             rdfs:label "side dish"@en-gb ;
             vs:term_status "testing" .


###  http://purl.org/ontology/fo/stages
fo:stages rdf:type owl:ObjectProperty ;
          rdfs:domain fo:Recipe ;
          rdfs:range fo:StageSequence ;
          rdfs:comment "The stages property relates a recipe to the sequence of stages it contains."@en-gb ;
          rdfs:isDefinedBy <http://purl.org/ontology/fo/> ;
          rdfs:label "stages"@en-gb ;
          vs:term_status "testing" .


###  http://purl.org/ontology/fo/starter
fo:starter rdf:type owl:ObjectProperty ;
           rdfs:domain fo:Menu ;
           rdfs:range fo:Recipe ;
           rdfs:comment "The starter property relates a menu to a recipe that may be served as a starter."@en-gb ;
           rdfs:isDefinedBy <http://purl.org/ontology/fo/> ;
           rdfs:label "starter"@en-gb ;
           vs:term_status "testing" .


#################################################################
#    Data properties
#################################################################

###  http://purl.org/dc/terms/alternative
dcterms:alternative rdf:type owl:DatatypeProperty ;
                    rdfs:subPropertyOf dcterms:title ;
                    rdfs:range rdfs:Literal .


###  http://purl.org/dc/terms/available
dcterms:available rdf:type owl:DatatypeProperty ;
                  rdfs:subPropertyOf dcterms:date ;
                  rdfs:range rdfs:Literal .


###  http://purl.org/dc/terms/bibliographicCitation
dcterms:bibliographicCitation rdf:type owl:DatatypeProperty ;
                              rdfs:subPropertyOf dcterms:identifier ;
                              rdfs:domain dcterms:BibliographicResource ;
                              rdfs:range rdfs:Literal .


###  http://purl.org/dc/terms/created
dcterms:created rdf:type owl:DatatypeProperty ;
                rdfs:subPropertyOf dcterms:date ;
                rdfs:range rdfs:Literal .


###  http://purl.org/dc/terms/date
dcterms:date rdf:type owl:DatatypeProperty ;
             rdfs:range rdfs:Literal .


###  http://purl.org/dc/terms/dateAccepted
dcterms:dateAccepted rdf:type owl:DatatypeProperty ;
                     rdfs:subPropertyOf dcterms:date ;
                     rdfs:range rdfs:Literal .


###  http://purl.org/dc/terms/dateCopyrighted
dcterms:dateCopyrighted rdf:type owl:DatatypeProperty ;
                        rdfs:subPropertyOf dcterms:date ;
                        rdfs:range rdfs:Literal .


###  http://purl.org/dc/terms/dateSubmitted
dcterms:dateSubmitted rdf:type owl:DatatypeProperty ;
                      rdfs:subPropertyOf dcterms:date ;
                      rdfs:range rdfs:Literal .


###  http://purl.org/dc/terms/identifier
dcterms:identifier rdf:type owl:DatatypeProperty ;
                   rdfs:range rdfs:Literal .


###  http://purl.org/dc/terms/issued
dcterms:issued rdf:type owl:DatatypeProperty ;
               rdfs:subPropertyOf dcterms:date ;
               rdfs:range rdfs:Literal .


###  http://purl.org/dc/terms/modified
dcterms:modified rdf:type owl:DatatypeProperty ;
                 rdfs:subPropertyOf dcterms:date ;
                 rdfs:range rdfs:Literal .


###  http://purl.org/dc/terms/title
dcterms:title rdf:type owl:DatatypeProperty ;
              rdfs:range rdfs:Literal .


###  http://purl.org/dc/terms/valid
dcterms:valid rdf:type owl:DatatypeProperty ;
              rdfs:subPropertyOf dcterms:date ;
              rdfs:range rdfs:Literal .


###  http://purl.org/ontology/fo/imperial_quantity
fo:imperial_quantity rdf:type owl:DatatypeProperty ;
                     rdfs:domain fo:Ingredient ;
                     rdfs:range xsd:string ;
                     rdfs:comment "A metric quantity provides a value and imperial unit in a human readable string for use in measuring out an ingredient."@en-gb ;
                     rdfs:isDefinedBy <http://purl.org/ontology/fo/> ;
                     rdfs:label "imperial quantity"@en-gb ;
                     vs:term_status "testing" .


###  http://purl.org/ontology/fo/instruction
fo:instruction rdf:type owl:DatatypeProperty ;
               rdfs:domain fo:Step ;
               rdfs:range xsd:string ;
               rdfs:comment "An instruction provides the human-readable text associated with a step in the method for a recipe."@en-gb ;
               rdfs:isDefinedBy <http://purl.org/ontology/fo/> ;
               rdfs:label "instruction"@en-gb ;
               vs:term_status "testing" .


###  http://purl.org/ontology/fo/metric_quantity
fo:metric_quantity rdf:type owl:DatatypeProperty ;
                   rdfs:domain fo:Ingredient ;
                   rdfs:range xsd:string ;
                   rdfs:comment "A metric quantity provides a value and metric unit in a human readable string for use in measuring out an ingredient."@en-gb ;
                   rdfs:isDefinedBy <http://purl.org/ontology/fo/> ;
                   rdfs:label "metric quantity"@en-gb ;
                   vs:term_status "testing" .


###  http://purl.org/ontology/fo/quantity
fo:quantity rdf:type owl:DatatypeProperty ;
            rdfs:domain fo:Ingredient ;
            rdfs:range xsd:nonNegativeInteger ;
            rdfs:comment "A quantity provides a non-negative integer quantity that can be used as a measure of the food stuff for the ingredient."@en-gb ;
            rdfs:isDefinedBy <http://purl.org/ontology/fo/> ;
            rdfs:label "quantity"@en-gb ;
            vs:term_status "testing" .


###  http://purl.org/ontology/fo/serves
fo:serves rdf:type owl:DatatypeProperty ;
          rdfs:domain fo:Recipe ;
          rdfs:range xsd:string ;
          rdfs:comment "The server property indicates what the recipe is intended to serve, this is often a human readable integer range such as '6-8'."@en-gb ;
          rdfs:isDefinedBy <http://purl.org/ontology/fo/> ;
          rdfs:label "serves"@en-gb ;
          vs:term_status "testing" .


#################################################################
#    Classes
#################################################################

###  http://purl.org/dc/dcam/VocabularyEncodingScheme
<http://purl.org/dc/dcam/VocabularyEncodingScheme> rdf:type owl:Class .


###  http://purl.org/dc/dcmitype/Collection
dctypes:Collection rdf:type owl:Class .


###  http://purl.org/dc/terms/Agent
dcterms:Agent rdf:type owl:Class .


###  http://purl.org/dc/terms/AgentClass
dcterms:AgentClass rdf:type owl:Class ;
                   rdfs:subClassOf rdfs:Class .


###  http://purl.org/dc/terms/BibliographicResource
dcterms:BibliographicResource rdf:type owl:Class .


###  http://purl.org/dc/terms/FileFormat
dcterms:FileFormat rdf:type owl:Class ;
                   rdfs:subClassOf dcterms:MediaType .


###  http://purl.org/dc/terms/Frequency
dcterms:Frequency rdf:type owl:Class .


###  http://purl.org/dc/terms/Jurisdiction
dcterms:Jurisdiction rdf:type owl:Class ;
                     rdfs:subClassOf dcterms:LocationPeriodOrJurisdiction .


###  http://purl.org/dc/terms/LicenseDocument
dcterms:LicenseDocument rdf:type owl:Class ;
                        rdfs:subClassOf dcterms:RightsStatement .


###  http://purl.org/dc/terms/LinguisticSystem
dcterms:LinguisticSystem rdf:type owl:Class .


###  http://purl.org/dc/terms/Location
dcterms:Location rdf:type owl:Class ;
                 rdfs:subClassOf dcterms:LocationPeriodOrJurisdiction .


###  http://purl.org/dc/terms/LocationPeriodOrJurisdiction
dcterms:LocationPeriodOrJurisdiction rdf:type owl:Class .


###  http://purl.org/dc/terms/MediaType
dcterms:MediaType rdf:type owl:Class ;
                  rdfs:subClassOf dcterms:MediaTypeOrExtent .


###  http://purl.org/dc/terms/MediaTypeOrExtent
dcterms:MediaTypeOrExtent rdf:type owl:Class .


###  http://purl.org/dc/terms/MethodOfAccrual
dcterms:MethodOfAccrual rdf:type owl:Class .


###  http://purl.org/dc/terms/MethodOfInstruction
dcterms:MethodOfInstruction rdf:type owl:Class .


###  http://purl.org/dc/terms/PeriodOfTime
dcterms:PeriodOfTime rdf:type owl:Class ;
                     rdfs:subClassOf dcterms:LocationPeriodOrJurisdiction .


###  http://purl.org/dc/terms/PhysicalMedium
dcterms:PhysicalMedium rdf:type owl:Class ;
                       rdfs:subClassOf dcterms:MediaType .


###  http://purl.org/dc/terms/PhysicalResource
dcterms:PhysicalResource rdf:type owl:Class .


###  http://purl.org/dc/terms/Policy
dcterms:Policy rdf:type owl:Class .


###  http://purl.org/dc/terms/ProvenanceStatement
dcterms:ProvenanceStatement rdf:type owl:Class .


###  http://purl.org/dc/terms/RightsStatement
dcterms:RightsStatement rdf:type owl:Class .


###  http://purl.org/dc/terms/SizeOrDuration
dcterms:SizeOrDuration rdf:type owl:Class ;
                       rdfs:subClassOf dcterms:MediaTypeOrExtent .


###  http://purl.org/dc/terms/Standard
dcterms:Standard rdf:type owl:Class .


###  http://purl.org/ontology/fo/Collection
fo:Collection rdf:type owl:Class ;
              rdfs:subClassOf dctypes:Collection ;
              rdfs:comment "A Collection is a group of recipes that are brought together because they have something in common. Some collections may result from automated queries such as all recipes that share a particular ingredient, other collections may be the result of editorial selection."@en-gb ;
              rdfs:isDefinedBy <http://purl.org/ontology/fo/> ;
              rdfs:label "Collection"@en-gb ;
              vs:term_status "testing" .


###  http://purl.org/ontology/fo/Course
fo:Course rdf:type owl:Class ;
          rdfs:comment "A Course is the sequence of a dish within a meal. For example a basic dinner party may consists of Starter, Main and Dessert courses."@en-gb ;
          rdfs:isDefinedBy <http://purl.org/ontology/fo/> ;
          rdfs:label "Course"@en-gb ;
          vs:term_status "testing" .


###  http://purl.org/ontology/fo/Cuisine
fo:Cuisine rdf:type owl:Class ;
           rdfs:comment "A Cuisine is a particular style of food, often based on a region. These classifications are often highly subjective."@en-gb ;
           rdfs:isDefinedBy <http://purl.org/ontology/fo/> ;
           rdfs:label "Cuisine"@en-gb ;
           vs:term_status "testing" .


###  http://purl.org/ontology/fo/Diet
fo:Diet rdf:type owl:Class ;
        rdfs:comment "A Diet is a way of selecting food that achieves a particular effect, such as eating in way that is pregnancy-friendly or avoiding foods that contain shellfish."@en-gb ;
        rdfs:isDefinedBy <http://purl.org/ontology/fo/> ;
        rdfs:label "Diet"@en-gb ;
        vs:term_status "testing" .


###  http://purl.org/ontology/fo/Food
fo:Food rdf:type owl:Class ;
        rdfs:comment "A Food is something that can be eaten. It may be a basic food such as salt or it may be the more complex result of another recipe, for example chicken stock. A recipe uses foods as part of ingredients and also produces foods to be eaten."@en-gb ;
        rdfs:isDefinedBy <http://purl.org/ontology/fo/> ;
        rdfs:label "Food"@en-gb ;
        vs:term_status "testing" .


###  http://purl.org/ontology/fo/Ingredient
fo:Ingredient rdf:type owl:Class .


###  http://purl.org/ontology/fo/IngredientList
fo:IngredientList rdf:type owl:Class ;
                  rdfs:subClassOf rdf:Seq ;
                  rdfs:comment "An IngredientList is a sequence (rdf:Seq) of ingredients in the order they should be listed in the recipe."@en-gb ;
                  rdfs:isDefinedBy <http://purl.org/ontology/fo/> ;
                  rdfs:label "IngredientList"@en-gb ;
                  vs:term_status "testing" .


###  http://purl.org/ontology/fo/Menu
fo:Menu rdf:type owl:Class ;
        rdfs:subClassOf fo:Collection ;
        rdfs:comment "A Menu is a collection of recipes, usually one or more per course, that have been selected to go well together. A Menu may also be related to a particular cuisine or occasion."@en-gb ;
        rdfs:isDefinedBy <http://purl.org/ontology/fo/> ;
        rdfs:label "Menu"@en-gb ;
        vs:term_status "testing" .


###  http://purl.org/ontology/fo/Method
fo:Method rdf:type owl:Class ;
          rdfs:subClassOf rdf:Seq ;
          rdfs:comment "A Method is the way in which ingredients are combined, using particular techniques, in order to produce a food. A method is part of a recipe and is also an rdf:Seq."@en-gb ;
          rdfs:isDefinedBy <http://purl.org/ontology/fo/> ;
          rdfs:label "Method"@en-gb ;
          vs:term_status "testing" .


###  http://purl.org/ontology/fo/Occasion
fo:Occasion rdf:type owl:Class ;
            rdfs:comment "An Occasion is a recognised event or type of event that a particular food may be suitable for. An exmaple of a particular occassion might be Chinese New Year, whereas a more general occassion might a birthday."@en-gb ;
            rdfs:isDefinedBy <http://purl.org/ontology/fo/> ;
            rdfs:label "Occasion"@en-gb ;
            vs:term_status "testing" .


###  http://purl.org/ontology/fo/Recipe
fo:Recipe rdf:type owl:Class .


###  http://purl.org/ontology/fo/Season
fo:Season rdf:type owl:Class ;
          rdfs:comment "A Season is a period of time that recurs annually during which a food is typically available or at its best."@en-gb ;
          rdfs:isDefinedBy <http://purl.org/ontology/fo/> ;
          rdfs:label "Season"@en-gb ;
          vs:term_status "testing" .


###  http://purl.org/ontology/fo/ShoppingCategory
fo:ShoppingCategory rdf:type owl:Class ;
                    rdfs:comment "A Shopping Category is a classification given to a food to indicate where it may be found when shopping."@en-gb ;
                    rdfs:isDefinedBy <http://purl.org/ontology/fo/> ;
                    rdfs:label "ShoppingCategory"@en-gb ;
                    vs:term_status "testing" .


###  http://purl.org/ontology/fo/Stage
fo:Stage rdf:type owl:Class ;
         rdfs:comment "A Stage is a part of a recipe that may have its own ingredient list and/or method. It allows the different parts of a multi-part recipe to be modelled seperately, yet as part of the same recipe."@en-gb ;
         rdfs:isDefinedBy <http://purl.org/ontology/fo/> ;
         rdfs:label "Stage"@en-gb ;
         vs:term_status "testing" .


###  http://purl.org/ontology/fo/StageSequence
fo:StageSequence rdf:type owl:Class ;
                 rdfs:subClassOf rdf:Seq ;
                 rdfs:comment "Where a recipe has a number of stage, for example where a recipe states 'for the sauce' a stage sequence provides a way to sequence the stages (rdf:Seq) into the desired order."@en-gb ;
                 rdfs:isDefinedBy <http://purl.org/ontology/fo/> ;
                 rdfs:label "StageSequence"@en-gb ;
                 vs:term_status "testing" .


###  http://purl.org/ontology/fo/Step
fo:Step rdf:type owl:Class ;
        rdfs:comment "A Step is the lowest level of instruction used in a recipe. A sequence of steps form a method."@en-gb ;
        rdfs:isDefinedBy <http://purl.org/ontology/fo/> ;
        rdfs:label "Step"@en-gb ;
        vs:term_status "testing" .


###  http://purl.org/ontology/fo/Technique
fo:Technique rdf:type owl:Class ;
             rdfs:comment "A Technique is a way of working with an ingredient to produce a desired effect, for example, whipping cream."@en-gb ;
             rdfs:isDefinedBy <http://purl.org/ontology/fo/> ;
             rdfs:label "Technique"@en-gb ;
             vs:term_status "testing" .


###  http://www.bbc.co.uk/ontologies/provenance/Ontology
provenance:Ontology rdf:type owl:Class .


###  http://www.w3.org/1999/02/22-rdf-syntax-ns#Seq
rdf:Seq rdf:type owl:Class .


#################################################################
#    Individuals
#################################################################

###  http://creativecommons.org/licenses/by/4.0#id
<http://creativecommons.org/licenses/by/4.0#id> rdf:type owl:NamedIndividual .


###  http://purl.org/dc/aboutdcmi#DCMI
<http://purl.org/dc/aboutdcmi#DCMI> rdf:type owl:NamedIndividual .


###  http://purl.org/dc/terms/
dcterms: rdf:type owl:NamedIndividual ;
         dcterms:publisher <http://purl.org/dc/aboutdcmi#DCMI> ;
         dcterms:modified "2012-06-14"^^xsd:date ;
         dcterms:title "DCMI Metadata Terms - other"@en .


###  http://purl.org/dc/terms/Agent
dcterms:Agent rdf:type owl:NamedIndividual ,
                       dcterms:AgentClass ;
              dcterms:issued "2008-01-14"^^xsd:date .


###  http://purl.org/dc/terms/AgentClass
dcterms:AgentClass rdf:type owl:NamedIndividual ;
                   dcterms:issued "2008-01-14"^^xsd:date ;
                   dcterms:modified "2012-06-14"^^xsd:date .


###  http://purl.org/dc/terms/BibliographicResource
dcterms:BibliographicResource rdf:type owl:NamedIndividual ;
                              dcterms:issued "2008-01-14"^^xsd:date .


###  http://purl.org/dc/terms/Box
dcterms:Box rdf:type owl:NamedIndividual ;
            dcterms:issued "2000-07-11"^^xsd:date ;
            dcterms:modified "2008-01-14"^^xsd:date .


###  http://purl.org/dc/terms/DCMIType
dcterms:DCMIType rdf:type owl:NamedIndividual ,
                          <http://purl.org/dc/dcam/VocabularyEncodingScheme> ;
                 dcterms:issued "2000-07-11"^^xsd:date ;
                 dcterms:modified "2012-06-14"^^xsd:date ;
                 dcterms:hasVersion <http://dublincore.org/usage/terms/history/#DCMIType-005> ;
                 rdfs:comment "The set of classes specified by the DCMI Type Vocabulary, used to categorize the nature or genre of the resource."@en ;
                 rdfs:isDefinedBy dcterms: ;
                 rdfs:label "DCMI Type Vocabulary"@en ;
                 rdfs:seeAlso dctypes: .


###  http://purl.org/dc/terms/DDC
dcterms:DDC rdf:type owl:NamedIndividual ,
                     <http://purl.org/dc/dcam/VocabularyEncodingScheme> ;
            dcterms:issued "2000-07-11"^^xsd:date ;
            dcterms:modified "2008-01-14"^^xsd:date ;
            dcterms:hasVersion <http://dublincore.org/usage/terms/history/#DDC-003> ;
            rdfs:comment "The set of conceptual resources specified by the Dewey Decimal Classification."@en ;
            rdfs:isDefinedBy dcterms: ;
            rdfs:label "DDC"@en ;
            rdfs:seeAlso <http://www.oclc.org/dewey/> .


###  http://purl.org/dc/terms/FileFormat
dcterms:FileFormat rdf:type owl:NamedIndividual ;
                   dcterms:issued "2008-01-14"^^xsd:date .


###  http://purl.org/dc/terms/Frequency
dcterms:Frequency rdf:type owl:NamedIndividual ;
                  dcterms:issued "2008-01-14"^^xsd:date .


###  http://purl.org/dc/terms/IMT
dcterms:IMT rdf:type owl:NamedIndividual ,
                     <http://purl.org/dc/dcam/VocabularyEncodingScheme> ;
            dcterms:issued "2000-07-11"^^xsd:date ;
            dcterms:modified "2008-01-14"^^xsd:date ;
            dcterms:hasVersion <http://dublincore.org/usage/terms/history/#IMT-004> ;
            rdfs:comment "The set of media types specified by the Internet Assigned Numbers Authority."@en ;
            rdfs:isDefinedBy dcterms: ;
            rdfs:label "IMT"@en ;
            rdfs:seeAlso <http://www.iana.org/assignments/media-types/> .


###  http://purl.org/dc/terms/ISO3166
dcterms:ISO3166 rdf:type owl:NamedIndividual ;
                dcterms:issued "2000-07-11"^^xsd:date ;
                dcterms:modified "2008-01-14"^^xsd:date .


###  http://purl.org/dc/terms/ISO639-2
dcterms:ISO639-2 rdf:type owl:NamedIndividual ;
                 dcterms:issued "2000-07-11"^^xsd:date ;
                 dcterms:modified "2008-01-14"^^xsd:date .


###  http://purl.org/dc/terms/ISO639-3
dcterms:ISO639-3 rdf:type owl:NamedIndividual ;
                 dcterms:issued "2008-01-14"^^xsd:date .


###  http://purl.org/dc/terms/Jurisdiction
dcterms:Jurisdiction rdf:type owl:NamedIndividual ;
                     dcterms:issued "2008-01-14"^^xsd:date .


###  http://purl.org/dc/terms/LCC
dcterms:LCC rdf:type owl:NamedIndividual ,
                     <http://purl.org/dc/dcam/VocabularyEncodingScheme> ;
            dcterms:issued "2000-07-11"^^xsd:date ;
            dcterms:modified "2008-01-14"^^xsd:date ;
            dcterms:hasVersion <http://dublincore.org/usage/terms/history/#LCC-003> ;
            rdfs:comment "The set of conceptual resources specified by the Library of Congress Classification."@en ;
            rdfs:isDefinedBy dcterms: ;
            rdfs:label "LCC"@en ;
            rdfs:seeAlso <http://lcweb.loc.gov/catdir/cpso/lcco/lcco.html> .


###  http://purl.org/dc/terms/LCSH
dcterms:LCSH rdf:type owl:NamedIndividual ,
                      <http://purl.org/dc/dcam/VocabularyEncodingScheme> ;
             dcterms:issued "2000-07-11"^^xsd:date ;
             dcterms:modified "2008-01-14"^^xsd:date ;
             dcterms:hasVersion <http://dublincore.org/usage/terms/history/#LCSH-003> ;
             rdfs:comment "The set of labeled concepts specified by the Library of Congress Subject Headings."@en ;
             rdfs:isDefinedBy dcterms: ;
             rdfs:label "LCSH"@en .


###  http://purl.org/dc/terms/LicenseDocument
dcterms:LicenseDocument rdf:type owl:NamedIndividual ;
                        dcterms:issued "2008-01-14"^^xsd:date .


###  http://purl.org/dc/terms/LinguisticSystem
dcterms:LinguisticSystem rdf:type owl:NamedIndividual ;
                         dcterms:issued "2008-01-14"^^xsd:date .


###  http://purl.org/dc/terms/Location
dcterms:Location rdf:type owl:NamedIndividual ;
                 dcterms:issued "2008-01-14"^^xsd:date .


###  http://purl.org/dc/terms/LocationPeriodOrJurisdiction
dcterms:LocationPeriodOrJurisdiction rdf:type owl:NamedIndividual ;
                                     dcterms:issued "2008-01-14"^^xsd:date .


###  http://purl.org/dc/terms/MESH
dcterms:MESH rdf:type owl:NamedIndividual ,
                      <http://purl.org/dc/dcam/VocabularyEncodingScheme> ;
             dcterms:issued "2000-07-11"^^xsd:date ;
             dcterms:modified "2008-01-14"^^xsd:date ;
             dcterms:hasVersion <http://dublincore.org/usage/terms/history/#MESH-003> ;
             rdfs:comment "The set of labeled concepts specified by the Medical Subject Headings."@en ;
             rdfs:isDefinedBy dcterms: ;
             rdfs:label "MeSH"@en ;
             rdfs:seeAlso <http://www.nlm.nih.gov/mesh/meshhome.html> .


###  http://purl.org/dc/terms/MediaType
dcterms:MediaType rdf:type owl:NamedIndividual ;
                  dcterms:issued "2008-01-14"^^xsd:date .


###  http://purl.org/dc/terms/MediaTypeOrExtent
dcterms:MediaTypeOrExtent rdf:type owl:NamedIndividual ;
                          dcterms:issued "2008-01-14"^^xsd:date .


###  http://purl.org/dc/terms/MethodOfAccrual
dcterms:MethodOfAccrual rdf:type owl:NamedIndividual ;
                        dcterms:issued "2008-01-14"^^xsd:date .


###  http://purl.org/dc/terms/MethodOfInstruction
dcterms:MethodOfInstruction rdf:type owl:NamedIndividual ;
                            dcterms:issued "2008-01-14"^^xsd:date .


###  http://purl.org/dc/terms/NLM
dcterms:NLM rdf:type owl:NamedIndividual ,
                     <http://purl.org/dc/dcam/VocabularyEncodingScheme> ;
            dcterms:issued "2005-06-13"^^xsd:date ;
            dcterms:modified "2008-01-14"^^xsd:date ;
            dcterms:hasVersion <http://dublincore.org/usage/terms/history/#NLM-002> ;
            rdfs:comment "The set of conceptual resources specified by the National Library of Medicine Classification."@en ;
            rdfs:isDefinedBy dcterms: ;
            rdfs:label "NLM"@en ;
            rdfs:seeAlso <http://wwwcf.nlm.nih.gov/class/> .


###  http://purl.org/dc/terms/Period
dcterms:Period rdf:type owl:NamedIndividual ;
               dcterms:issued "2000-07-11"^^xsd:date ;
               dcterms:modified "2008-01-14"^^xsd:date .


###  http://purl.org/dc/terms/PeriodOfTime
dcterms:PeriodOfTime rdf:type owl:NamedIndividual ;
                     dcterms:issued "2008-01-14"^^xsd:date .


###  http://purl.org/dc/terms/PhysicalMedium
dcterms:PhysicalMedium rdf:type owl:NamedIndividual ;
                       dcterms:issued "2008-01-14"^^xsd:date .


###  http://purl.org/dc/terms/PhysicalResource
dcterms:PhysicalResource rdf:type owl:NamedIndividual ;
                         dcterms:issued "2008-01-14"^^xsd:date .


###  http://purl.org/dc/terms/Point
dcterms:Point rdf:type owl:NamedIndividual ;
              dcterms:issued "2000-07-11"^^xsd:date ;
              dcterms:modified "2008-01-14"^^xsd:date .


###  http://purl.org/dc/terms/Policy
dcterms:Policy rdf:type owl:NamedIndividual ;
               dcterms:issued "2008-01-14"^^xsd:date .


###  http://purl.org/dc/terms/ProvenanceStatement
dcterms:ProvenanceStatement rdf:type owl:NamedIndividual ;
                            dcterms:issued "2008-01-14"^^xsd:date .


###  http://purl.org/dc/terms/RFC1766
dcterms:RFC1766 rdf:type owl:NamedIndividual ;
                dcterms:issued "2000-07-11"^^xsd:date ;
                dcterms:modified "2008-01-14"^^xsd:date .


###  http://purl.org/dc/terms/RFC3066
dcterms:RFC3066 rdf:type owl:NamedIndividual ;
                dcterms:issued "2002-07-13"^^xsd:date ;
                dcterms:modified "2008-01-14"^^xsd:date .


###  http://purl.org/dc/terms/RFC4646
dcterms:RFC4646 rdf:type owl:NamedIndividual ;
                dcterms:issued "2008-01-14"^^xsd:date .


###  http://purl.org/dc/terms/RFC5646
dcterms:RFC5646 rdf:type owl:NamedIndividual ;
                dcterms:issued "2010-10-11"^^xsd:date .


###  http://purl.org/dc/terms/RightsStatement
dcterms:RightsStatement rdf:type owl:NamedIndividual ;
                        dcterms:issued "2008-01-14"^^xsd:date .


###  http://purl.org/dc/terms/SizeOrDuration
dcterms:SizeOrDuration rdf:type owl:NamedIndividual ;
                       dcterms:issued "2008-01-14"^^xsd:date .


###  http://purl.org/dc/terms/Standard
dcterms:Standard rdf:type owl:NamedIndividual ;
                 dcterms:issued "2008-01-14"^^xsd:date .


###  http://purl.org/dc/terms/TGN
dcterms:TGN rdf:type owl:NamedIndividual ,
                     <http://purl.org/dc/dcam/VocabularyEncodingScheme> ;
            dcterms:issued "2000-07-11"^^xsd:date ;
            dcterms:modified "2008-01-14"^^xsd:date ;
            dcterms:hasVersion <http://dublincore.org/usage/terms/history/#TGN-003> ;
            rdfs:comment "The set of places specified by the Getty Thesaurus of Geographic Names."@en ;
            rdfs:isDefinedBy dcterms: ;
            rdfs:label "TGN"@en ;
            rdfs:seeAlso <http://www.getty.edu/research/tools/vocabulary/tgn/index.html> .


###  http://purl.org/dc/terms/UDC
dcterms:UDC rdf:type owl:NamedIndividual ,
                     <http://purl.org/dc/dcam/VocabularyEncodingScheme> ;
            dcterms:issued "2000-07-11"^^xsd:date ;
            dcterms:modified "2008-01-14"^^xsd:date ;
            dcterms:hasVersion <http://dublincore.org/usage/terms/history/#UDC-003> ;
            rdfs:comment "The set of conceptual resources specified by the Universal Decimal Classification."@en ;
            rdfs:isDefinedBy dcterms: ;
            rdfs:label "UDC"@en ;
            rdfs:seeAlso <http://www.udcc.org/> .


###  http://purl.org/dc/terms/URI
dcterms:URI rdf:type owl:NamedIndividual ;
            dcterms:issued "2000-07-11"^^xsd:date ;
            dcterms:modified "2008-01-14"^^xsd:date .


###  http://purl.org/dc/terms/W3CDTF
dcterms:W3CDTF rdf:type owl:NamedIndividual ;
               dcterms:issued "2000-07-11"^^xsd:date ;
               dcterms:modified "2008-01-14"^^xsd:date .


###  http://purl.org/dc/terms/abstract
dcterms:abstract rdf:type owl:NamedIndividual ;
                 dcterms:issued "2000-07-11"^^xsd:date ;
                 dcterms:modified "2008-01-14"^^xsd:date .


###  http://purl.org/dc/terms/accessRights
dcterms:accessRights rdf:type owl:NamedIndividual ;
                     dcterms:issued "2003-02-15"^^xsd:date ;
                     dcterms:modified "2008-01-14"^^xsd:date .


###  http://purl.org/dc/terms/accrualMethod
dcterms:accrualMethod rdf:type owl:NamedIndividual ;
                      dcterms:issued "2005-06-13"^^xsd:date ;
                      dcterms:modified "2010-10-11"^^xsd:date .


###  http://purl.org/dc/terms/accrualPeriodicity
dcterms:accrualPeriodicity rdf:type owl:NamedIndividual ;
                           dcterms:issued "2005-06-13"^^xsd:date ;
                           dcterms:modified "2010-10-11"^^xsd:date .


###  http://purl.org/dc/terms/accrualPolicy
dcterms:accrualPolicy rdf:type owl:NamedIndividual ;
                      dcterms:issued "2005-06-13"^^xsd:date ;
                      dcterms:modified "2010-10-11"^^xsd:date .


###  http://purl.org/dc/terms/alternative
dcterms:alternative rdf:type owl:NamedIndividual ;
                    dcterms:issued "2000-07-11"^^xsd:date ;
                    dcterms:modified "2010-10-11"^^xsd:date .


###  http://purl.org/dc/terms/audience
dcterms:audience rdf:type owl:NamedIndividual ;
                 dcterms:issued "2001-05-21"^^xsd:date ;
                 dcterms:modified "2008-01-14"^^xsd:date .


###  http://purl.org/dc/terms/available
dcterms:available rdf:type owl:NamedIndividual ;
                  dcterms:issued "2000-07-11"^^xsd:date ;
                  dcterms:modified "2008-01-14"^^xsd:date .


###  http://purl.org/dc/terms/bibliographicCitation
dcterms:bibliographicCitation rdf:type owl:NamedIndividual ;
                              dcterms:issued "2003-02-15"^^xsd:date ;
                              dcterms:modified "2008-01-14"^^xsd:date .


###  http://purl.org/dc/terms/conformsTo
dcterms:conformsTo rdf:type owl:NamedIndividual ;
                   dcterms:issued "2001-05-21"^^xsd:date ;
                   dcterms:modified "2008-01-14"^^xsd:date .


###  http://purl.org/dc/terms/contributor
dcterms:contributor rdf:type owl:NamedIndividual ;
                    dcterms:issued "2008-01-14"^^xsd:date ;
                    dcterms:modified "2010-10-11"^^xsd:date .


###  http://purl.org/dc/terms/coverage
dcterms:coverage rdf:type owl:NamedIndividual ;
                 dcterms:issued "2008-01-14"^^xsd:date ;
                 dcterms:modified "2008-01-14"^^xsd:date .


###  http://purl.org/dc/terms/created
dcterms:created rdf:type owl:NamedIndividual ;
                dcterms:issued "2000-07-11"^^xsd:date ;
                dcterms:modified "2008-01-14"^^xsd:date .


###  http://purl.org/dc/terms/creator
dcterms:creator rdf:type owl:NamedIndividual ;
                dcterms:issued "2008-01-14"^^xsd:date ;
                dcterms:modified "2010-10-11"^^xsd:date .


###  http://purl.org/dc/terms/date
dcterms:date rdf:type owl:NamedIndividual ;
             dcterms:issued "2008-01-14"^^xsd:date ;
             dcterms:modified "2008-01-14"^^xsd:date .


###  http://purl.org/dc/terms/dateAccepted
dcterms:dateAccepted rdf:type owl:NamedIndividual ;
                     dcterms:issued "2002-07-13"^^xsd:date ;
                     dcterms:modified "2008-01-14"^^xsd:date .


###  http://purl.org/dc/terms/dateCopyrighted
dcterms:dateCopyrighted rdf:type owl:NamedIndividual ;
                        dcterms:issued "2002-07-13"^^xsd:date ;
                        dcterms:modified "2008-01-14"^^xsd:date .


###  http://purl.org/dc/terms/dateSubmitted
dcterms:dateSubmitted rdf:type owl:NamedIndividual ;
                      dcterms:issued "2002-07-13"^^xsd:date ;
                      dcterms:modified "2008-01-14"^^xsd:date .


###  http://purl.org/dc/terms/description
dcterms:description rdf:type owl:NamedIndividual ;
                    dcterms:issued "2008-01-14"^^xsd:date ;
                    dcterms:modified "2008-01-14"^^xsd:date .


###  http://purl.org/dc/terms/educationLevel
dcterms:educationLevel rdf:type owl:NamedIndividual ;
                       dcterms:issued "2002-07-13"^^xsd:date ;
                       dcterms:modified "2008-01-14"^^xsd:date .


###  http://purl.org/dc/terms/extent
dcterms:extent rdf:type owl:NamedIndividual ;
               dcterms:issued "2000-07-11"^^xsd:date ;
               dcterms:modified "2008-01-14"^^xsd:date .


###  http://purl.org/dc/terms/format
dcterms:format rdf:type owl:NamedIndividual ;
               dcterms:issued "2008-01-14"^^xsd:date ;
               dcterms:modified "2008-01-14"^^xsd:date .


###  http://purl.org/dc/terms/hasFormat
dcterms:hasFormat rdf:type owl:NamedIndividual ;
                  dcterms:issued "2000-07-11"^^xsd:date ;
                  dcterms:modified "2008-01-14"^^xsd:date .


###  http://purl.org/dc/terms/hasPart
dcterms:hasPart rdf:type owl:NamedIndividual ;
                dcterms:issued "2000-07-11"^^xsd:date ;
                dcterms:modified "2008-01-14"^^xsd:date .


###  http://purl.org/dc/terms/hasVersion
dcterms:hasVersion rdf:type owl:NamedIndividual ;
                   dcterms:issued "2000-07-11"^^xsd:date ;
                   dcterms:modified "2008-01-14"^^xsd:date .


###  http://purl.org/dc/terms/identifier
dcterms:identifier rdf:type owl:NamedIndividual ;
                   dcterms:issued "2008-01-14"^^xsd:date ;
                   dcterms:modified "2008-01-14"^^xsd:date .


###  http://purl.org/dc/terms/instructionalMethod
dcterms:instructionalMethod rdf:type owl:NamedIndividual ;
                            dcterms:issued "2005-06-13"^^xsd:date ;
                            dcterms:modified "2008-01-14"^^xsd:date .


###  http://purl.org/dc/terms/isFormatOf
dcterms:isFormatOf rdf:type owl:NamedIndividual ;
                   dcterms:issued "2000-07-11"^^xsd:date ;
                   dcterms:modified "2008-01-14"^^xsd:date .


###  http://purl.org/dc/terms/isPartOf
dcterms:isPartOf rdf:type owl:NamedIndividual ;
                 dcterms:issued "2000-07-11"^^xsd:date ;
                 dcterms:modified "2008-01-14"^^xsd:date .


###  http://purl.org/dc/terms/isReferencedBy
dcterms:isReferencedBy rdf:type owl:NamedIndividual ;
                       dcterms:issued "2000-07-11"^^xsd:date ;
                       dcterms:modified "2008-01-14"^^xsd:date .


###  http://purl.org/dc/terms/isReplacedBy
dcterms:isReplacedBy rdf:type owl:NamedIndividual ;
                     dcterms:issued "2000-07-11"^^xsd:date ;
                     dcterms:modified "2008-01-14"^^xsd:date .


###  http://purl.org/dc/terms/isRequiredBy
dcterms:isRequiredBy rdf:type owl:NamedIndividual ;
                     dcterms:issued "2000-07-11"^^xsd:date ;
                     dcterms:modified "2008-01-14"^^xsd:date .


###  http://purl.org/dc/terms/isVersionOf
dcterms:isVersionOf rdf:type owl:NamedIndividual ;
                    dcterms:issued "2000-07-11"^^xsd:date ;
                    dcterms:modified "2008-01-14"^^xsd:date .


###  http://purl.org/dc/terms/issued
dcterms:issued rdf:type owl:NamedIndividual ,
                        owl:DatatypeProperty ;
               dcterms:issued "2000-07-11"^^xsd:date ;
               dcterms:modified "2008-01-14"^^xsd:date .


###  http://purl.org/dc/terms/language
dcterms:language rdf:type owl:NamedIndividual ;
                 dcterms:issued "2008-01-14"^^xsd:date ;
                 dcterms:modified "2008-01-14"^^xsd:date .


###  http://purl.org/dc/terms/license
dcterms:license rdf:type owl:NamedIndividual ;
                dcterms:issued "2004-06-14"^^xsd:date ;
                dcterms:modified "2008-01-14"^^xsd:date .


###  http://purl.org/dc/terms/mediator
dcterms:mediator rdf:type owl:NamedIndividual ;
                 dcterms:issued "2001-05-21"^^xsd:date ;
                 dcterms:modified "2008-01-14"^^xsd:date .


###  http://purl.org/dc/terms/medium
dcterms:medium rdf:type owl:NamedIndividual ;
               dcterms:issued "2000-07-11"^^xsd:date ;
               dcterms:modified "2008-01-14"^^xsd:date .


###  http://purl.org/dc/terms/modified
dcterms:modified rdf:type owl:NamedIndividual ;
                 dcterms:issued "2000-07-11"^^xsd:date ;
                 rdf:type owl:DatatypeProperty ;
                 dcterms:modified "2008-01-14"^^xsd:date .


###  http://purl.org/dc/terms/provenance
dcterms:provenance rdf:type owl:NamedIndividual ;
                   dcterms:issued "2004-09-20"^^xsd:date ;
                   dcterms:modified "2008-01-14"^^xsd:date .


###  http://purl.org/dc/terms/publisher
dcterms:publisher rdf:type owl:NamedIndividual ;
                  dcterms:issued "2008-01-14"^^xsd:date ;
                  dcterms:modified "2010-10-11"^^xsd:date .


###  http://purl.org/dc/terms/references
dcterms:references rdf:type owl:NamedIndividual ;
                   dcterms:issued "2000-07-11"^^xsd:date ;
                   dcterms:modified "2008-01-14"^^xsd:date .


###  http://purl.org/dc/terms/relation
dcterms:relation rdf:type owl:NamedIndividual ;
                 dcterms:issued "2008-01-14"^^xsd:date ;
                 dcterms:modified "2008-01-14"^^xsd:date .


###  http://purl.org/dc/terms/replaces
dcterms:replaces rdf:type owl:NamedIndividual ;
                 dcterms:issued "2000-07-11"^^xsd:date ;
                 dcterms:modified "2008-01-14"^^xsd:date .


###  http://purl.org/dc/terms/requires
dcterms:requires rdf:type owl:NamedIndividual ;
                 dcterms:issued "2000-07-11"^^xsd:date ;
                 dcterms:modified "2008-01-14"^^xsd:date .


###  http://purl.org/dc/terms/rights
dcterms:rights rdf:type owl:NamedIndividual ;
               dcterms:issued "2008-01-14"^^xsd:date ;
               dcterms:modified "2008-01-14"^^xsd:date .


###  http://purl.org/dc/terms/rightsHolder
dcterms:rightsHolder rdf:type owl:NamedIndividual ;
                     dcterms:issued "2004-06-14"^^xsd:date ;
                     dcterms:modified "2008-01-14"^^xsd:date .


###  http://purl.org/dc/terms/source
dcterms:source rdf:type owl:NamedIndividual ;
               dcterms:issued "2008-01-14"^^xsd:date ;
               dcterms:modified "2008-01-14"^^xsd:date .


###  http://purl.org/dc/terms/spatial
dcterms:spatial rdf:type owl:NamedIndividual ;
                dcterms:issued "2000-07-11"^^xsd:date ;
                dcterms:modified "2008-01-14"^^xsd:date .


###  http://purl.org/dc/terms/subject
dcterms:subject rdf:type owl:NamedIndividual ;
                dcterms:issued "2008-01-14"^^xsd:date ;
                dcterms:modified "2012-06-14"^^xsd:date .


###  http://purl.org/dc/terms/tableOfContents
dcterms:tableOfContents rdf:type owl:NamedIndividual ;
                        dcterms:issued "2000-07-11"^^xsd:date ;
                        dcterms:modified "2008-01-14"^^xsd:date .


###  http://purl.org/dc/terms/temporal
dcterms:temporal rdf:type owl:NamedIndividual ;
                 dcterms:issued "2000-07-11"^^xsd:date ;
                 dcterms:modified "2008-01-14"^^xsd:date .


###  http://purl.org/dc/terms/title
dcterms:title rdf:type owl:NamedIndividual ;
              dcterms:issued "2008-01-14"^^xsd:date ;
              dcterms:modified "2010-10-11"^^xsd:date .


###  http://purl.org/dc/terms/type
dcterms:type rdf:type owl:NamedIndividual ;
             dcterms:issued "2008-01-14"^^xsd:date ;
             dcterms:modified "2008-01-14"^^xsd:date .


###  http://purl.org/dc/terms/valid
dcterms:valid rdf:type owl:NamedIndividual ;
              dcterms:issued "2000-07-11"^^xsd:date ;
              dcterms:modified "2008-01-14"^^xsd:date .


###  http://purl.org/ontology/fo/
<http://purl.org/ontology/fo/> rdf:type owl:NamedIndividual ,
                                        provenance:Ontology ;
                               dcterms:license <http://creativecommons.org/licenses/by/4.0#id> ;
                               foaf:maker <http://purl.org/ontology/fo/#andrew> ,
                                          <http://purl.org/ontology/fo/#oliver> ,
                                          <http://purl.org/ontology/fo/#philip> ,
                                          <http://purl.org/ontology/fo/#rija> ,
                                          <http://purl.org/ontology/fo/#rob> ;
                               dcterms:created "2011-07-08"^^xsd:date ;
                               dcterms:title "Food Ontology"@en-gb .


###  http://purl.org/ontology/fo/Ingredient
fo:Ingredient rdf:type owl:NamedIndividual ;
              owl:sameAs v:Ingredient .


###  http://purl.org/ontology/fo/Recipe
fo:Recipe rdf:type owl:NamedIndividual ;
          owl:sameAs v:Recipe .


###  http://purl.org/ontology/fo/#andrew
<http://purl.org/ontology/fo/#andrew> rdf:type owl:NamedIndividual ,
                                               foaf:Person ;
                                      foaf:name "Andrew Robinson" .


###  http://purl.org/ontology/fo/#oliver
<http://purl.org/ontology/fo/#oliver> rdf:type owl:NamedIndividual ,
                                               foaf:Person ;
                                      foaf:name "Oliver Bartlett" .


###  http://purl.org/ontology/fo/#philip
<http://purl.org/ontology/fo/#philip> rdf:type owl:NamedIndividual ,
                                               foaf:Person ;
                                      foaf:name "Philip Lamond" .


###  http://purl.org/ontology/fo/#rija
<http://purl.org/ontology/fo/#rija> rdf:type owl:NamedIndividual ,
                                             foaf:Person ;
                                    foaf:name "Rija Menage" .


###  http://purl.org/ontology/fo/#rob
<http://purl.org/ontology/fo/#rob> rdf:type owl:NamedIndividual ,
                                            foaf:Person ;
                                   foaf:name "Rob Styles" .


###  http://rdf.data-vocabulary.org/#Ingredient
v:Ingredient rdf:type owl:NamedIndividual .


###  http://rdf.data-vocabulary.org/#Recipe
v:Recipe rdf:type owl:NamedIndividual .


#################################################################
#    Annotations
#################################################################

dc: dcterms:publisher <http://purl.org/dc/aboutdcmi#DCMI> ;
    dcterms:title "Dublin Core Metadata Element Set, Version 1.1"@en ;
    dcterms:modified "2012-06-14"^^xsd:date .


dcterms:Agent rdfs:label "Agent"@en ;
              rdfs:isDefinedBy dcterms: ;
              rdfs:comment "A resource that acts or has the power to act."@en ;
              dcterms:description "Examples of Agent include person, organization, and software agent."@en ;
              dcterms:hasVersion <http://dublincore.org/usage/terms/history/#Agent-001> .


dcterms:AgentClass rdfs:isDefinedBy dcterms: ;
                   rdfs:label "Agent Class"@en ;
                   rdfs:comment "A group of agents."@en ;
                   dcterms:description "Examples of Agent Class include groups seen as classes, such as students, women, charities, lecturers."@en ;
                   dcterms:hasVersion <http://dublincore.org/usage/terms/history/#AgentClass-003> .


dcterms:BibliographicResource rdfs:isDefinedBy dcterms: ;
                              dcterms:hasVersion <http://dublincore.org/usage/terms/history/#BibliographicResource-001> ;
                              rdfs:comment "A book, article, or other documentary resource."@en ;
                              rdfs:label "Bibliographic Resource"@en .


dcterms:Box rdfs:comment "The set of regions in space defined by their geographic coordinates according to the DCMI Box Encoding Scheme."@en ;
            rdfs:isDefinedBy dcterms: ;
            rdfs:label "DCMI Box"@en ;
            rdfs:seeAlso <http://dublincore.org/documents/dcmi-box/> ;
            dcterms:hasVersion <http://dublincore.org/usage/terms/history/#Box-003> .


dcterms:FileFormat dcterms:description "Examples include the formats defined by the list of Internet Media Types."@en ;
                   dcterms:hasVersion <http://dublincore.org/usage/terms/history/#FileFormat-001> ;
                   rdfs:label "File Format"@en ;
                   rdfs:comment "A digital resource format."@en ;
                   rdfs:isDefinedBy dcterms: .


dcterms:Frequency rdfs:label "Frequency"@en ;
                  dcterms:hasVersion <http://dublincore.org/usage/terms/history/#Frequency-001> ;
                  rdfs:isDefinedBy dcterms: ;
                  rdfs:comment "A rate at which something recurs."@en .


dcterms:ISO3166 rdfs:comment "The set of codes listed in ISO 3166-1 for the representation of names of countries."@en ;
                rdfs:isDefinedBy dcterms: ;
                dcterms:hasVersion <http://dublincore.org/usage/terms/history/#ISO3166-004> ;
                rdfs:label "ISO 3166"@en ;
                rdfs:seeAlso <http://www.iso.org/iso/en/prods-services/iso3166ma/02iso-3166-code-lists/list-en1.html> .


dcterms:ISO639-2 rdfs:seeAlso <http://lcweb.loc.gov/standards/iso639-2/langhome.html> ;
                 rdfs:comment "The three-letter alphabetic codes listed in ISO639-2 for the representation of names of languages."@en ;
                 rdfs:isDefinedBy dcterms: ;
                 rdfs:label "ISO 639-2"@en ;
                 dcterms:hasVersion <http://dublincore.org/usage/terms/history/#ISO639-2-003> .


dcterms:ISO639-3 rdfs:comment "The set of three-letter codes listed in ISO 639-3 for the representation of names of languages."@en ;
                 rdfs:label "ISO 639-3"@en ;
                 rdfs:isDefinedBy dcterms: ;
                 dcterms:hasVersion <http://dublincore.org/usage/terms/history/#ISO639-3-001> ;
                 rdfs:seeAlso <http://www.sil.org/iso639-3/> .


dcterms:Jurisdiction dcterms:hasVersion <http://dublincore.org/usage/terms/history/#Jurisdiction-001> ;
                     rdfs:label "Jurisdiction"@en ;
                     rdfs:isDefinedBy dcterms: ;
                     rdfs:comment "The extent or range of judicial, law enforcement, or other authority."@en .


dcterms:LicenseDocument rdfs:label "License Document"@en ;
                        rdfs:isDefinedBy dcterms: ;
                        rdfs:comment "A legal document giving official permission to do something with a Resource."@en ;
                        dcterms:hasVersion <http://dublincore.org/usage/terms/history/#LicenseDocument-001> .


dcterms:LinguisticSystem dcterms:hasVersion <http://dublincore.org/usage/terms/history/#LinguisticSystem-001> ;
                         dcterms:description "Examples include written, spoken, sign, and computer languages."@en ;
                         rdfs:isDefinedBy dcterms: ;
                         rdfs:comment "A system of signs, symbols, sounds, gestures, or rules used in communication."@en ;
                         rdfs:label "Linguistic System"@en .


dcterms:Location dcterms:hasVersion <http://dublincore.org/usage/terms/history/#Location-001> ;
                 rdfs:label "Location"@en ;
                 rdfs:isDefinedBy dcterms: ;
                 rdfs:comment "A spatial region or named place."@en .


dcterms:LocationPeriodOrJurisdiction rdfs:label "Location, Period, or Jurisdiction"@en ;
                                     rdfs:comment "A location, period of time, or jurisdiction."@en ;
                                     rdfs:isDefinedBy dcterms: ;
                                     dcterms:hasVersion <http://dublincore.org/usage/terms/history/#LocationPeriodOrJurisdiction-001> .


dcterms:MediaType rdfs:comment "A file format or physical medium."@en ;
                  rdfs:label "Media Type"@en ;
                  rdfs:isDefinedBy dcterms: ;
                  dcterms:hasVersion <http://dublincore.org/usage/terms/history/#MediaType-001> .


dcterms:MediaTypeOrExtent rdfs:isDefinedBy dcterms: ;
                          rdfs:comment "A media type or extent."@en ;
                          rdfs:label "Media Type or Extent"@en ;
                          dcterms:hasVersion <http://dublincore.org/usage/terms/history/#MediaTypeOrExtent-001> .


dcterms:MethodOfAccrual rdfs:isDefinedBy dcterms: ;
                        rdfs:comment "A method by which resources are added to a collection."@en ;
                        dcterms:hasVersion <http://dublincore.org/usage/terms/history/#MethodOfAccrual-001> ;
                        rdfs:label "Method of Accrual"@en .


dcterms:MethodOfInstruction rdfs:label "Method of Instruction"@en ;
                            rdfs:comment "A process that is used to engender knowledge, attitudes, and skills."@en ;
                            dcterms:hasVersion <http://dublincore.org/usage/terms/history/#MethodOfInstruction-001> ;
                            rdfs:isDefinedBy dcterms: .


dcterms:Period rdfs:comment "The set of time intervals defined by their limits according to the DCMI Period Encoding Scheme."@en ;
               rdfs:seeAlso <http://dublincore.org/documents/dcmi-period/> ;
               rdfs:label "DCMI Period"@en ;
               rdfs:isDefinedBy dcterms: ;
               dcterms:hasVersion <http://dublincore.org/usage/terms/history/#Period-003> .


dcterms:PeriodOfTime rdfs:comment "An interval of time that is named or defined by its start and end dates."@en ;
                     dcterms:hasVersion <http://dublincore.org/usage/terms/history/#PeriodOfTime-001> ;
                     rdfs:isDefinedBy dcterms: ;
                     rdfs:label "Period of Time"@en .


dcterms:PhysicalMedium dcterms:hasVersion <http://dublincore.org/usage/terms/history/#PhysicalMedium-001> ;
                       dcterms:description "Examples include paper, canvas, or DVD."@en ;
                       rdfs:label "Physical Medium"@en ;
                       rdfs:isDefinedBy dcterms: ;
                       rdfs:comment "A physical material or carrier."@en .


dcterms:PhysicalResource rdfs:isDefinedBy dcterms: ;
                         rdfs:comment "A material thing."@en ;
                         dcterms:hasVersion <http://dublincore.org/usage/terms/history/#PhysicalResource-001> ;
                         rdfs:label "Physical Resource"@en .


dcterms:Point rdfs:comment "The set of points in space defined by their geographic coordinates according to the DCMI Point Encoding Scheme."@en ;
              rdfs:label "DCMI Point"@en ;
              dcterms:hasVersion <http://dublincore.org/usage/terms/history/#Point-003> ;
              rdfs:seeAlso <http://dublincore.org/documents/dcmi-point/> ;
              rdfs:isDefinedBy dcterms: .


dcterms:Policy rdfs:isDefinedBy dcterms: ;
               rdfs:label "Policy"@en ;
               rdfs:comment "A plan or course of action by an authority, intended to influence and determine decisions, actions, and other matters."@en ;
               dcterms:hasVersion <http://dublincore.org/usage/terms/history/#Policy-001> .


dcterms:ProvenanceStatement rdfs:label "Provenance Statement"@en ;
                            rdfs:isDefinedBy dcterms: ;
                            dcterms:hasVersion <http://dublincore.org/usage/terms/history/#ProvenanceStatement-001> ;
                            rdfs:comment "A statement of any changes in ownership and custody of a resource since its creation that are significant for its authenticity, integrity, and interpretation."@en .


dcterms:RFC1766 rdfs:isDefinedBy dcterms: ;
                rdfs:seeAlso <http://www.ietf.org/rfc/rfc1766.txt> ;
                dcterms:hasVersion <http://dublincore.org/usage/terms/history/#RFC1766-003> ;
                rdfs:comment "The set of tags, constructed according to RFC 1766, for the identification of languages."@en ;
                rdfs:label "RFC 1766"@en .


dcterms:RFC3066 rdfs:label "RFC 3066"@en ;
                rdfs:isDefinedBy dcterms: ;
                dcterms:description "RFC 3066 has been obsoleted by RFC 4646."@en ;
                rdfs:comment "The set of tags constructed according to RFC 3066 for the identification of languages."@en ;
                rdfs:seeAlso <http://www.ietf.org/rfc/rfc3066.txt> ;
                dcterms:hasVersion <http://dublincore.org/usage/terms/history/#RFC3066-002> .


dcterms:RFC4646 dcterms:description "RFC 4646 obsoletes RFC 3066."@en ;
                dcterms:hasVersion <http://dublincore.org/usage/terms/history/#RFC4646-001> ;
                rdfs:seeAlso <http://www.ietf.org/rfc/rfc4646.txt> ;
                rdfs:isDefinedBy dcterms: ;
                rdfs:comment "The set of tags constructed according to RFC 4646 for the identification of languages."@en ;
                rdfs:label "RFC 4646"@en .


dcterms:RFC5646 rdfs:seeAlso <http://www.ietf.org/rfc/rfc5646.txt> ;
                dcterms:hasVersion <http://dublincore.org/usage/terms/history/#RFC5646-001> ;
                rdfs:comment "The set of tags constructed according to RFC 5646 for the identification of languages."@en ;
                rdfs:label "RFC 5646"@en ;
                dcterms:description "RFC 5646 obsoletes RFC 4646."@en ;
                rdfs:isDefinedBy dcterms: .


dcterms:RightsStatement rdfs:label "Rights Statement"@en ;
                        rdfs:isDefinedBy dcterms: ;
                        rdfs:comment "A statement about the intellectual property rights (IPR) held in or over a Resource, a legal document giving official permission to do something with a resource, or a statement about access rights."@en ;
                        dcterms:hasVersion <http://dublincore.org/usage/terms/history/#RightsStatement-001> .


dcterms:SizeOrDuration rdfs:label "Size or Duration"@en ;
                       dcterms:hasVersion <http://dublincore.org/usage/terms/history/#SizeOrDuration-001> ;
                       dcterms:description "Examples include a number of pages, a specification of length, width, and breadth, or a period in hours, minutes, and seconds."@en ;
                       rdfs:comment "A dimension or extent, or a time taken to play or execute."@en ;
                       rdfs:isDefinedBy dcterms: .


dcterms:Standard rdfs:comment "A basis for comparison; a reference point against which other things can be evaluated."@en ;
                 rdfs:label "Standard"@en ;
                 rdfs:isDefinedBy dcterms: ;
                 dcterms:hasVersion <http://dublincore.org/usage/terms/history/#Standard-001> .


dcterms:URI rdfs:isDefinedBy dcterms: ;
            rdfs:comment "The set of identifiers constructed according to the generic syntax for Uniform Resource Identifiers as specified by the Internet Engineering Task Force."@en ;
            rdfs:seeAlso <http://www.ietf.org/rfc/rfc3986.txt> ;
            dcterms:hasVersion <http://dublincore.org/usage/terms/history/#URI-003> ;
            rdfs:label "URI"@en .


dcterms:W3CDTF rdfs:label "W3C-DTF"@en ;
               rdfs:comment "The set of dates and times constructed according to the W3C Date and Time Formats Specification."@en ;
               rdfs:isDefinedBy dcterms: ;
               dcterms:hasVersion <http://dublincore.org/usage/terms/history/#W3CDTF-003> ;
               rdfs:seeAlso <http://www.w3.org/TR/NOTE-datetime> .


dcterms:abstract rdfs:label "Abstract"@en ;
                 dcterms:hasVersion <http://dublincore.org/usage/terms/history/#abstract-003> ;
                 rdfs:comment "A summary of the resource."@en ;
                 rdfs:isDefinedBy dcterms: .


dcterms:accessRights dcterms:description "Access Rights may include information regarding access or restrictions based on privacy, security, or other policies."@en ;
                     rdfs:comment "Information about who can access the resource or an indication of its security status."@en ;
                     rdfs:label "Access Rights"@en ;
                     dcterms:hasVersion <http://dublincore.org/usage/terms/history/#accessRights-002> ;
                     rdfs:isDefinedBy dcterms: .


dcterms:accrualMethod rdfs:label "Accrual Method"@en ;
                      dcterms:hasVersion <http://dublincore.org/usage/terms/history/#accrualMethod-003> ;
                      rdfs:comment "The method by which items are added to a collection."@en ;
                      rdfs:isDefinedBy dcterms: .


dcterms:accrualPeriodicity dcterms:hasVersion <http://dublincore.org/usage/terms/history/#accrualPeriodicity-003> ;
                           rdfs:label "Accrual Periodicity"@en ;
                           rdfs:comment "The frequency with which items are added to a collection."@en ;
                           rdfs:isDefinedBy dcterms: .


dcterms:accrualPolicy rdfs:isDefinedBy dcterms: ;
                      rdfs:comment "The policy governing the addition of items to a collection."@en ;
                      dcterms:hasVersion <http://dublincore.org/usage/terms/history/#accrualPolicy-003> ;
                      rdfs:label "Accrual Policy"@en .


dcterms:alternative rdfs:comment "An alternative name for the resource."@en ;
                    rdfs:isDefinedBy dcterms: ;
                    dcterms:hasVersion <http://dublincore.org/usage/terms/history/#alternative-003> ;
                    dcterms:description "The distinction between titles and alternative titles is application-specific."@en ;
                    rdfs:label "Alternative Title"@en .


dcterms:audience rdfs:comment "A class of entity for whom the resource is intended or useful."@en ;
                 dcterms:hasVersion <http://dublincore.org/usage/terms/history/#audience-003> ;
                 rdfs:label "Audience"@en ;
                 rdfs:isDefinedBy dcterms: .


dcterms:available rdfs:isDefinedBy dcterms: ;
                  rdfs:label "Date Available"@en ;
                  rdfs:comment "Date (often a range) that the resource became or will become available."@en ;
                  dcterms:hasVersion <http://dublincore.org/usage/terms/history/#available-003> .


dcterms:bibliographicCitation dcterms:description "Recommended practice is to include sufficient bibliographic detail to identify the resource as unambiguously as possible."@en ;
                              rdfs:label "Bibliographic Citation"@en ;
                              dcterms:hasVersion <http://dublincore.org/usage/terms/history/#bibliographicCitation-002> ;
                              rdfs:comment "A bibliographic reference for the resource."@en ;
                              rdfs:isDefinedBy dcterms: .


dcterms:conformsTo rdfs:isDefinedBy dcterms: ;
                   rdfs:label "Conforms To"@en ;
                   rdfs:comment "An established standard to which the described resource conforms."@en ;
                   dcterms:hasVersion <http://dublincore.org/usage/terms/history/#conformsTo-003> .


dcterms:contributor rdfs:comment "An entity responsible for making contributions to the resource."@en ;
                    rdfs:isDefinedBy dcterms: ;
                    dcterms:description "Examples of a Contributor include a person, an organization, or a service."@en ;
                    dcterms:hasVersion <http://dublincore.org/usage/terms/history/#contributorT-001> ;
                    rdfs:label "Contributor"@en .


dcterms:coverage rdfs:isDefinedBy dcterms: ;
                 dcterms:hasVersion <http://dublincore.org/usage/terms/history/#coverageT-001> ;
                 rdfs:label "Coverage"@en ;
                 dcterms:description "Spatial topic and spatial applicability may be a named place or a location specified by its geographic coordinates. Temporal topic may be a named period, date, or date range. A jurisdiction may be a named administrative entity or a geographic place to which the resource applies. Recommended best practice is to use a controlled vocabulary such as the Thesaurus of Geographic Names [TGN]. Where appropriate, named places or time periods can be used in preference to numeric identifiers such as sets of coordinates or date ranges."@en ;
                 rdfs:comment "The spatial or temporal topic of the resource, the spatial applicability of the resource, or the jurisdiction under which the resource is relevant."@en .


dcterms:created rdfs:isDefinedBy dcterms: ;
                rdfs:comment "Date of creation of the resource."@en ;
                dcterms:hasVersion <http://dublincore.org/usage/terms/history/#created-003> ;
                rdfs:label "Date Created"@en .


dcterms:creator rdfs:comment "An entity primarily responsible for making the resource."@en ;
                dcterms:hasVersion <http://dublincore.org/usage/terms/history/#creatorT-002> ;
                rdfs:isDefinedBy dcterms: ;
                rdfs:label "Creator"@en ;
                dcterms:description "Examples of a Creator include a person, an organization, or a service."@en .


dcterms:date rdfs:isDefinedBy dcterms: ;
             rdfs:comment "A point or period of time associated with an event in the lifecycle of the resource."@en ;
             dcterms:hasVersion <http://dublincore.org/usage/terms/history/#dateT-001> ;
             dcterms:description "Date may be used to express temporal information at any level of granularity.  Recommended best practice is to use an encoding scheme, such as the W3CDTF profile of ISO 8601 [W3CDTF]."@en ;
             rdfs:label "Date"@en .


dcterms:dateAccepted dcterms:hasVersion <http://dublincore.org/usage/terms/history/#dateAccepted-002> ;
                     dcterms:description "Examples of resources to which a Date Accepted may be relevant are a thesis (accepted by a university department) or an article (accepted by a journal)."@en ;
                     rdfs:comment "Date of acceptance of the resource."@en ;
                     rdfs:label "Date Accepted"@en ;
                     rdfs:isDefinedBy dcterms: .


dcterms:dateCopyrighted rdfs:isDefinedBy dcterms: ;
                        rdfs:label "Date Copyrighted"@en ;
                        rdfs:comment "Date of copyright."@en ;
                        dcterms:hasVersion <http://dublincore.org/usage/terms/history/#dateCopyrighted-002> .


dcterms:dateSubmitted rdfs:comment "Date of submission of the resource."@en ;
                      dcterms:description "Examples of resources to which a Date Submitted may be relevant are a thesis (submitted to a university department) or an article (submitted to a journal)."@en ;
                      dcterms:hasVersion <http://dublincore.org/usage/terms/history/#dateSubmitted-002> ;
                      rdfs:label "Date Submitted"@en ;
                      rdfs:isDefinedBy dcterms: .


dcterms:description rdfs:label "Description"@en ;
                    rdfs:isDefinedBy dcterms: ;
                    dcterms:hasVersion <http://dublincore.org/usage/terms/history/#descriptionT-001> ;
                    rdfs:comment "An account of the resource."@en ;
                    rdf:type owl:AnnotationProperty ;
                    dcterms:description "Description may include but is not limited to: an abstract, a table of contents, a graphical representation, or a free-text account of the resource."@en .


dcterms:educationLevel rdfs:isDefinedBy dcterms: ;
                       rdfs:label "Audience Education Level"@en ;
                       rdfs:comment "A class of entity, defined in terms of progression through an educational or training context, for which the described resource is intended."@en ;
                       dcterms:hasVersion <http://dublincore.org/usage/terms/history/#educationLevel-002> .


dcterms:extent rdfs:isDefinedBy dcterms: ;
               rdfs:comment "The size or duration of the resource."@en ;
               dcterms:hasVersion <http://dublincore.org/usage/terms/history/#extent-003> ;
               rdfs:label "Extent"@en .


dcterms:format dcterms:hasVersion <http://dublincore.org/usage/terms/history/#formatT-001> ;
               rdfs:comment "The file format, physical medium, or dimensions of the resource."@en ;
               dcterms:description "Examples of dimensions include size and duration. Recommended best practice is to use a controlled vocabulary such as the list of Internet Media Types [MIME]."@en ;
               rdfs:isDefinedBy dcterms: ;
               rdfs:label "Format"@en .


dcterms:hasFormat skos:note "This term is intended to be used with non-literal values as defined in the DCMI Abstract Model (http://dublincore.org/documents/abstract-model/).  As of December 2007, the DCMI Usage Board is seeking a way to express this intention with a formal range declaration."@en ;
                  rdfs:isDefinedBy dcterms: ;
                  dcterms:hasVersion <http://dublincore.org/usage/terms/history/#hasFormat-003> ;
                  rdfs:label "Has Format"@en ;
                  rdfs:comment "A related resource that is substantially the same as the pre-existing described resource, but in another format."@en .


dcterms:hasPart rdfs:isDefinedBy dcterms: ;
                skos:note "This term is intended to be used with non-literal values as defined in the DCMI Abstract Model (http://dublincore.org/documents/abstract-model/).  As of December 2007, the DCMI Usage Board is seeking a way to express this intention with a formal range declaration."@en ;
                rdfs:label "Has Part"@en ;
                rdfs:comment "A related resource that is included either physically or logically in the described resource."@en ;
                dcterms:hasVersion <http://dublincore.org/usage/terms/history/#hasPart-003> .


dcterms:hasVersion rdf:type owl:AnnotationProperty ;
                   dcterms:hasVersion <http://dublincore.org/usage/terms/history/#hasVersion-003> ;
                   rdfs:isDefinedBy dcterms: ;
                   rdfs:comment "A related resource that is a version, edition, or adaptation of the described resource."@en ;
                   skos:note "This term is intended to be used with non-literal values as defined in the DCMI Abstract Model (http://dublincore.org/documents/abstract-model/).  As of December 2007, the DCMI Usage Board is seeking a way to express this intention with a formal range declaration."@en ;
                   rdfs:label "Has Version"@en .


dcterms:identifier dcterms:hasVersion <http://dublincore.org/usage/terms/history/#identifierT-001> ;
                   rdfs:isDefinedBy dcterms: ;
                   dcterms:description "Recommended best practice is to identify the resource by means of a string conforming to a formal identification system. "@en ;
                   rdfs:comment "An unambiguous reference to the resource within a given context."@en ;
                   rdfs:label "Identifier"@en .


dcterms:instructionalMethod dcterms:description "Instructional Method will typically include ways of presenting instructional materials or conducting instructional activities, patterns of learner-to-learner and learner-to-instructor interactions, and mechanisms by which group and individual levels of learning are measured.  Instructional methods include all aspects of the instruction and learning processes from planning and implementation through evaluation and feedback."@en ;
                            rdfs:label "Instructional Method"@en ;
                            rdfs:comment "A process, used to engender knowledge, attitudes and skills, that the described resource is designed to support."@en ;
                            dcterms:hasVersion <http://dublincore.org/usage/terms/history/#instructionalMethod-002> ;
                            rdfs:isDefinedBy dcterms: .


dcterms:isFormatOf dcterms:hasVersion <http://dublincore.org/usage/terms/history/#isFormatOf-003> ;
                   rdfs:comment "A related resource that is substantially the same as the described resource, but in another format."@en ;
                   skos:note "This term is intended to be used with non-literal values as defined in the DCMI Abstract Model (http://dublincore.org/documents/abstract-model/).  As of December 2007, the DCMI Usage Board is seeking a way to express this intention with a formal range declaration."@en ;
                   rdfs:label "Is Format Of"@en ;
                   rdfs:isDefinedBy dcterms: .


dcterms:isPartOf rdfs:label "Is Part Of"@en ;
                 dcterms:hasVersion <http://dublincore.org/usage/terms/history/#isPartOf-003> ;
                 skos:note "This term is intended to be used with non-literal values as defined in the DCMI Abstract Model (http://dublincore.org/documents/abstract-model/).  As of December 2007, the DCMI Usage Board is seeking a way to express this intention with a formal range declaration."@en ;
                 rdfs:isDefinedBy dcterms: ;
                 rdfs:comment "A related resource in which the described resource is physically or logically included."@en .


dcterms:isReferencedBy rdfs:label "Is Referenced By"@en ;
                       rdfs:comment "A related resource that references, cites, or otherwise points to the described resource."@en ;
                       rdfs:isDefinedBy dcterms: ;
                       skos:note "This term is intended to be used with non-literal values as defined in the DCMI Abstract Model (http://dublincore.org/documents/abstract-model/).  As of December 2007, the DCMI Usage Board is seeking a way to express this intention with a formal range declaration."@en ;
                       dcterms:hasVersion <http://dublincore.org/usage/terms/history/#isReferencedBy-003> .


dcterms:isReplacedBy rdfs:isDefinedBy dcterms: ;
                     rdfs:label "Is Replaced By"@en ;
                     rdfs:comment "A related resource that supplants, displaces, or supersedes the described resource."@en ;
                     skos:note "This term is intended to be used with non-literal values as defined in the DCMI Abstract Model (http://dublincore.org/documents/abstract-model/).  As of December 2007, the DCMI Usage Board is seeking a way to express this intention with a formal range declaration."@en ;
                     dcterms:hasVersion <http://dublincore.org/usage/terms/history/#isReplacedBy-003> .


dcterms:isRequiredBy rdfs:isDefinedBy dcterms: ;
                     skos:note "This term is intended to be used with non-literal values as defined in the DCMI Abstract Model (http://dublincore.org/documents/abstract-model/).  As of December 2007, the DCMI Usage Board is seeking a way to express this intention with a formal range declaration."@en ;
                     rdfs:label "Is Required By"@en ;
                     dcterms:hasVersion <http://dublincore.org/usage/terms/history/#isRequiredBy-003> ;
                     rdfs:comment "A related resource that requires the described resource to support its function, delivery, or coherence."@en .


dcterms:isVersionOf rdfs:label "Is Version Of"@en ;
                    rdfs:isDefinedBy dcterms: ;
                    rdfs:comment "A related resource of which the described resource is a version, edition, or adaptation."@en ;
                    skos:note "This term is intended to be used with non-literal values as defined in the DCMI Abstract Model (http://dublincore.org/documents/abstract-model/).  As of December 2007, the DCMI Usage Board is seeking a way to express this intention with a formal range declaration."@en ;
                    dcterms:hasVersion <http://dublincore.org/usage/terms/history/#isVersionOf-003> ;
                    dcterms:description "Changes in version imply substantive changes in content rather than differences in format."@en .


dcterms:issued rdfs:comment "Date of formal issuance (e.g., publication) of the resource."@en ;
               rdfs:isDefinedBy dcterms: ;
               dcterms:hasVersion <http://dublincore.org/usage/terms/history/#issued-003> ;
               rdfs:label "Date Issued"@en .


dcterms:language rdfs:label "Language"@en ;
                 dcterms:hasVersion <http://dublincore.org/usage/terms/history/#languageT-001> ;
                 rdfs:isDefinedBy dcterms: ;
                 dcterms:description "Recommended best practice is to use a controlled vocabulary such as RFC 4646 [RFC4646]."@en ;
                 rdfs:comment "A language of the resource."@en .


dcterms:license rdfs:label "License"@en ;
                rdfs:comment "A legal document giving official permission to do something with the resource."@en ;
                dcterms:hasVersion <http://dublincore.org/usage/terms/history/#license-002> ;
                rdfs:isDefinedBy dcterms: .


dcterms:mediator dcterms:description "In an educational context, a mediator might be a parent, teacher, teaching assistant, or care-giver."@en ;
                 rdfs:comment "An entity that mediates access to the resource and for whom the resource is intended or useful."@en ;
                 dcterms:hasVersion <http://dublincore.org/usage/terms/history/#mediator-003> ;
                 rdfs:isDefinedBy dcterms: ;
                 rdfs:label "Mediator"@en .


dcterms:medium rdfs:isDefinedBy dcterms: ;
               rdfs:label "Medium"@en ;
               rdfs:comment "The material or physical carrier of the resource."@en ;
               dcterms:hasVersion <http://dublincore.org/usage/terms/history/#medium-003> .


dcterms:modified rdfs:isDefinedBy dcterms: ;
                 rdfs:label "Date Modified"@en ;
                 dcterms:hasVersion <http://dublincore.org/usage/terms/history/#modified-003> ;
                 rdfs:comment "Date on which the resource was changed."@en .


dcterms:provenance rdfs:comment "A statement of any changes in ownership and custody of the resource since its creation that are significant for its authenticity, integrity, and interpretation."@en ;
                   rdfs:isDefinedBy dcterms: ;
                   dcterms:description "The statement may include a description of any changes successive custodians made to the resource."@en ;
                   dcterms:hasVersion <http://dublincore.org/usage/terms/history/#provenance-002> ;
                   rdfs:label "Provenance"@en .


dcterms:publisher rdfs:label "Publisher"@en ;
                  dcterms:hasVersion <http://dublincore.org/usage/terms/history/#publisherT-001> ;
                  dcterms:description "Examples of a Publisher include a person, an organization, or a service."@en ;
                  rdfs:isDefinedBy dcterms: ;
                  rdfs:comment "An entity responsible for making the resource available."@en .


dcterms:references rdfs:comment "A related resource that is referenced, cited, or otherwise pointed to by the described resource."@en ;
                   rdfs:label "References"@en ;
                   dcterms:hasVersion <http://dublincore.org/usage/terms/history/#references-003> ;
                   skos:note "This term is intended to be used with non-literal values as defined in the DCMI Abstract Model (http://dublincore.org/documents/abstract-model/).  As of December 2007, the DCMI Usage Board is seeking a way to express this intention with a formal range declaration."@en ;
                   rdfs:isDefinedBy dcterms: .


dcterms:relation skos:note "This term is intended to be used with non-literal values as defined in the DCMI Abstract Model (http://dublincore.org/documents/abstract-model/).  As of December 2007, the DCMI Usage Board is seeking a way to express this intention with a formal range declaration."@en ;
                 rdfs:isDefinedBy dcterms: ;
                 dcterms:hasVersion <http://dublincore.org/usage/terms/history/#relationT-001> ;
                 rdfs:label "Relation"@en ;
                 dcterms:description "Recommended best practice is to identify the related resource by means of a string conforming to a formal identification system. "@en ;
                 rdfs:comment "A related resource."@en .


dcterms:replaces skos:note "This term is intended to be used with non-literal values as defined in the DCMI Abstract Model (http://dublincore.org/documents/abstract-model/).  As of December 2007, the DCMI Usage Board is seeking a way to express this intention with a formal range declaration."@en ;
                 rdfs:label "Replaces"@en ;
                 dcterms:hasVersion <http://dublincore.org/usage/terms/history/#replaces-003> ;
                 rdfs:comment "A related resource that is supplanted, displaced, or superseded by the described resource."@en ;
                 rdfs:isDefinedBy dcterms: .


dcterms:requires dcterms:hasVersion <http://dublincore.org/usage/terms/history/#requires-003> ;
                 rdfs:label "Requires"@en ;
                 rdfs:comment "A related resource that is required by the described resource to support its function, delivery, or coherence."@en ;
                 rdfs:isDefinedBy dcterms: ;
                 skos:note "This term is intended to be used with non-literal values as defined in the DCMI Abstract Model (http://dublincore.org/documents/abstract-model/).  As of December 2007, the DCMI Usage Board is seeking a way to express this intention with a formal range declaration."@en .


dcterms:rights rdfs:isDefinedBy dcterms: ;
               rdfs:label "Rights"@en ;
               rdfs:comment "Information about rights held in and over the resource."@en ;
               dcterms:hasVersion <http://dublincore.org/usage/terms/history/#rightsT-001> ;
               dcterms:description "Typically, rights information includes a statement about various property rights associated with the resource, including intellectual property rights."@en .


dcterms:rightsHolder dcterms:hasVersion <http://dublincore.org/usage/terms/history/#rightsHolder-002> ;
                     rdfs:isDefinedBy dcterms: ;
                     rdfs:comment "A person or organization owning or managing rights over the resource."@en ;
                     rdfs:label "Rights Holder"@en .


dcterms:source rdfs:label "Source"@en ;
               skos:note "This term is intended to be used with non-literal values as defined in the DCMI Abstract Model (http://dublincore.org/documents/abstract-model/).  As of December 2007, the DCMI Usage Board is seeking a way to express this intention with a formal range declaration."@en ;
               rdfs:isDefinedBy dcterms: ;
               dcterms:hasVersion <http://dublincore.org/usage/terms/history/#sourceT-001> ;
               dcterms:description "The described resource may be derived from the related resource in whole or in part. Recommended best practice is to identify the related resource by means of a string conforming to a formal identification system."@en ;
               rdfs:comment "A related resource from which the described resource is derived."@en .


dcterms:spatial rdfs:label "Spatial Coverage"@en ;
                rdfs:isDefinedBy dcterms: ;
                rdfs:comment "Spatial characteristics of the resource."@en ;
                dcterms:hasVersion <http://dublincore.org/usage/terms/history/#spatial-003> .


dcterms:subject dcterms:hasVersion <http://dublincore.org/usage/terms/history/#subjectT-002> ;
                skos:note "This term is intended to be used with non-literal values as defined in the DCMI Abstract Model (http://dublincore.org/documents/abstract-model/).  As of December 2007, the DCMI Usage Board is seeking a way to express this intention with a formal range declaration."@en ;
                rdfs:label "Subject"@en ;
                rdfs:comment "The topic of the resource."@en ;
                dcterms:description "Typically, the subject will be represented using keywords, key phrases, or classification codes. Recommended best practice is to use a controlled vocabulary."@en ;
                rdfs:isDefinedBy dcterms: .


dcterms:tableOfContents rdfs:comment "A list of subunits of the resource."@en ;
                        rdfs:isDefinedBy dcterms: ;
                        rdfs:label "Table Of Contents"@en ;
                        dcterms:hasVersion <http://dublincore.org/usage/terms/history/#tableOfContents-003> .


dcterms:temporal rdfs:label "Temporal Coverage"@en ;
                 dcterms:hasVersion <http://dublincore.org/usage/terms/history/#temporal-003> ;
                 rdfs:comment "Temporal characteristics of the resource."@en ;
                 rdfs:isDefinedBy dcterms: .


dcterms:title rdfs:label "Title"@en ;
              rdfs:comment "A name given to the resource."@en ;
              dcterms:hasVersion <http://dublincore.org/usage/terms/history/#titleT-002> ;
              rdfs:isDefinedBy dcterms: .


dcterms:type rdfs:isDefinedBy dcterms: ;
             dcterms:description "Recommended best practice is to use a controlled vocabulary such as the DCMI Type Vocabulary [DCMITYPE]. To describe the file format, physical medium, or dimensions of the resource, use the Format element."@en ;
             rdfs:comment "The nature or genre of the resource."@en ;
             rdfs:label "Type"@en ;
             dcterms:hasVersion <http://dublincore.org/usage/terms/history/#typeT-001> .


dcterms:valid rdfs:comment "Date (often a range) of validity of a resource."@en ;
              rdfs:label "Date Valid"@en ;
              rdfs:isDefinedBy dcterms: ;
              dcterms:hasVersion <http://dublincore.org/usage/terms/history/#valid-003> .


fo:Ingredient rdfs:isDefinedBy <http://purl.org/ontology/fo/> ;
              rdfs:comment "An Ingredient is the combination of a quantity and a food, giving the amount of something that should be used in the recipe."@en-gb ;
              vs:term_status "testing" ;
              rdfs:label "Ingredient"@en-gb .


fo:Recipe vs:term_status "testing" ;
          rdfs:isDefinedBy <http://purl.org/ontology/fo/> ;
          rdfs:label "Recipe"@en-gb ;
          rdfs:comment "A Recipe is a combination of ingredients and a method, created by a chef, that produces a food."@en-gb .


###  Generated by the OWL API (version 4.5.9.2019-02-01T07:24:44Z) https://github.com/owlcs/owlapi
